wip

Matroid/Extremal/Covers.lean
@@ -8,14 +8,21 @@ import Matroid.Flat.LowRank
 import Matroid.ForMathlib.Topology.ENat
 import Matroid.ForMathlib.Minimal
 import Mathlib.Data.Set.Card.Arithmetic
+import Matroid.Uniform.Basic
+import Matroid.Uniform.Paving
+import Matroid.Uniform.Finite
+import Matroid.Uniform.Minor
+
 
 set_option linter.style.longLine false
 
 variable {α : Type*} {M N M' : Matroid α} {I F X Y F' F₀ F₁ F₂ P L H H₁ H₂ H' B C D K : Set α}
   {e f : α} {l r : ℕ} {a k : ℕ∞} {T : Set (Set α)} {ι : Type*} {i j : ι}
-  {P P' : Matroid α → Set α → Prop}
+  {P P' : Set α → Prop}
 
 open Set
+
+section General
 
 /-- `T.IsCover X P` means that `T` is a collection of sets with union `X`,
 each satisfying property `P`.-/
@@ -24,146 +31,42 @@ structure Set.IsCover (T : Set (Set α)) (X : Set α) (P : Set α → Prop) : Pr
   sUnion_eq : ⋃₀ T = X
   pProp : ∀ F ∈ T, P F
 
-noncomputable def Set.coverNumber (X : Set α) (P : Set α → Prop) : ℕ∞ :=
-  ⨅ (T : Set (Set α)) (_ : T.IsCover X P), T.encard
+lemma Set.IsCover.subset (h : T.IsCover X P) (hY : Y ∈ T) : Y ⊆ X := by
+  grw [← h.sUnion_eq, ← subset_sUnion_of_mem hY]
 
-lemma coverNumber_mono (X : Set α) {P Q : Set α → Prop} (hPQ : ∀ Y ⊆ X, P Y → Q Y) :
-    X.coverNumber Q ≤ X.coverNumber P := by
-  simp only [coverNumber, le_iInf_iff]
-  refine fun T hT ↦ iInf₂_le T ⟨hT.1, fun F hF ↦ hPQ _ ?_ (hT.2 F hF)⟩
+def Set.hasCover_with (X : Set α) (P : Set α → Prop) : Prop :=
+    ∃ T, IsCover T X P
 
-
-
-
-namespace Matroid
-
-def IsRankCover (M : Matroid α) (T : Set (Set α)) (X : Set α) (k : ℕ∞) :=
-    T.IsCover X (fun A ↦ M.eRk A ≤ k)
-
-
-
-section General
-
-
-
-
-@[mk_iff]
-structure IsCover (M : Matroid α) (P : Matroid α → Set α → Prop) (T : Set (Set α)) : Prop where
-  sUnion_eq : ⋃₀ T = M.E
-  pProp : ∀ F ∈ T, P M F
-
-lemma IsCover.subset_ground (h : M.IsCover P T) (hX : X ∈ T) : X ⊆ M.E := by
-  grw [← h.sUnion_eq, ← subset_sUnion_of_mem hX]
-
--- monotone
--- PCover iff ∀ e, ∃ X ∈ T, e ∈ X
-
---Monotone under restriction
-def IsMRProp (P : Matroid α → Set α → Prop) : Prop :=
-    ∀ M : Matroid α, ∀ F : Set α, ∀ Y : Set α, Y ⊆ F → P (M ↾ F) Y → P M Y
-
---Monotone under subset
-def IsMSProp (P : Matroid α → Set α → Prop) : Prop :=
-    ∀ M : Matroid α, ∀ F : Set α, ∀ Y : Set α, Y ⊆ F → P M F → P M Y
-
--- --Minor union different prop. I think I want something different
--- def IsMUProp (P : Matroid α → Set α → Prop) (P' : Matroid α → Set α → Prop) : Prop :=
---     ∀ M : Matroid α, ∀ X : Set α, ∀ Y : Set α, P (M ／ X) Y → P' M (Y ∪ X)
-
---Minor monotono
-def IsMMProp (P : Matroid α → Set α → Prop) (P' : Matroid α → Set α → Prop) : Prop :=
-    --∀ M : Matroid α, ∀ X : Set α, ∀ Y : Set α, P (M ／ X) Y → P' M (Y ∪ X)
-    ∀ N, N ≤m M → ∀ Y, Y ⊆ N.E → P N Y → P' M Y
-
--- M has a cover with respect to prop P
-def hasCover_with (M : Matroid α) (P : Matroid α → Set α → Prop) : Prop :=
-    ∃ T, M.IsCover P T
-
-lemma Cover_Nonempt_iff :
-    M.hasCover_with P ↔ {T | M.IsCover P T}.Nonempty := by
+lemma Cover_Nonempt_iff {X : Set α} :
+    X.hasCover_with P ↔ {T | IsCover T X P }.Nonempty := by
   refine ⟨ fun a ↦ Nonempty.mono (fun ⦃a⦄ a_1 ↦ a_1) a , fun a ↦ ((fun a_1 ↦ a) ∘ fun a ↦ α) α ⟩
 
-lemma IsCover.nonempty [M.Nonempty] (h : M.IsCover P T) : T.Nonempty := by
+lemma Set.IsCover.nonempty (h : T.IsCover X P) (hX : X.Nonempty) : T.Nonempty := by
   rw [nonempty_iff_empty_ne]
   rintro rfl
-  simp [isCover_iff, eq_comm, M.ground_nonempty.ne_empty] at h
+  simp [isCover_iff, eq_comm] at h
+  simp_all only [Set.not_nonempty_empty]
 
-lemma IsCover.one_le [M.Nonempty] (h : M.IsCover P T) : 1 ≤ T.encard := by
+lemma IsCover.one_le (h : T.IsCover X P ) (hX : X.Nonempty) : 1 ≤ T.encard := by
   simp only [one_le_encard_iff_nonempty]
-  exact nonempty h
+  exact h.nonempty hX
 
-noncomputable def coverNumber (M : Matroid α) (P : Matroid α → Set α → Prop) : ℕ∞ :=
-    sInf (encard '' {T | M.IsCover P T})
+-- --Monotono subset
+-- def IsMRProp (P : Set α → Prop) : Prop :=
+--     ∀ F : Set α, ∀ Y : Set α, Y ⊆ F → P Y → P F
 
-lemma coverNumber_eq_iInf (M : Matroid α) (P : Matroid α → Set α → Prop) :
-    M.coverNumber P = ⨅ T ∈ {T | M.IsCover P T}, T.encard := by
-  exact sInf_image
+-- -- def IsMRProp (P : Matroid α → Set α → Prop) : Prop :=
+-- --     ∀ M : Matroid α, ∀ F : Set α, ∀ Y : Set α, Y ⊆ F → P (M ↾ F) Y → P M Y
 
-lemma IsCover.coverNumber_le {T} (h : M.IsCover P T) : M.coverNumber P ≤ T.encard := by
-  grw [coverNumber_eq_iInf]
-  exact biInf_le encard h
+-- --Monotone under subset
+-- def IsMSProp (P : Set α → Prop) : Prop :=
+--     ∀ F : Set α, ∀ Y : Set α, Y ⊆ F → P F → P Y
 
-lemma exists_mincover_NE {M : Matroid α} {P : Matroid α → Set α → Prop}
-    (hn : {T | M.IsCover P T}.Nonempty) :
-    ∃ T, M.IsCover P T ∧ T.encard = M.coverNumber P := by
-  simpa using csInf_mem <| hn.image encard
-
-lemma exists_min_cover {M : Matroid α} {P : Matroid α → Set α → Prop} (hP : M.hasCover_with P) :
-    ∃ T, M.IsCover P T ∧ T.encard = M.coverNumber P := by
-  simpa using csInf_mem <| (Cover_Nonempt_iff.1 hP ).image encard
-
-lemma exists_cover (M : Matroid α) (P : Matroid α → Set α → Prop) :
-    M.coverNumber P = ⊤ ∨ ∃ T, M.IsCover P T ∧ T.encard = M.coverNumber P := by
-  obtain h0 | h := {T | M.IsCover P T}.eq_empty_or_nonempty
-  · simp [coverNumber_eq_iInf, h0]
-  right
-  simpa using csInf_mem <| h.image encard
-
-lemma coverNumer_positive [M.Nonempty] (P : Matroid α → Set α → Prop) :
-    1 ≤ M.coverNumber P := by
-  by_contra hc
-  have h1 := ENat.lt_one_iff_eq_zero.mp (Std.not_le.mp hc)
-  obtain ht | ⟨T, hT, hTe ⟩ := exists_cover M P
-  · rw [h1] at ht
-    simp only [ENat.zero_ne_top] at ht
-  have := hT.nonempty
-  grind
-
-lemma IsCover.cover_fun {M : Matroid α} {P' : Matroid α → Set α → Prop} (hP' : IsMRProp P')
-    (hcover : M.IsCover P T)
-    (f : Set α → Set (Set α) )
-    (hfun : ∀ X ∈ T, (M ↾ X).IsCover P' (f X)) :
-    M.IsCover P' ( ⋃ X ∈ T, f X ):= by
-  refine ⟨ ?_, ?_ ⟩
-  · rw[←hcover.sUnion_eq]
-    refine ext ?_
-    intro e
-    refine ⟨ ?_, ?_ ⟩
-    · intro he
-      simp only [ mem_sUnion, mem_iUnion] at he
-      obtain ⟨T', ⟨ X, ⟨hX, hT'X ⟩ ⟩, hee ⟩ := he
-      simp only [mem_sUnion]
-      refine ⟨ X ,⟨ hX , mem_of_subset_of_mem ((hfun X hX).subset_ground hT'X ) hee  ⟩ ⟩
-    intro he
-    simp only [mem_sUnion] at he
-    obtain ⟨X, hXT, heX⟩ := he
-    simp only [mem_sUnion, mem_iUnion]
-    have h1 : e ∈ (M ↾ ↑X).E := by exact mem_of_subset_of_mem (fun ⦃a⦄ a_1 ↦ a_1) heX
-    rw[←(hfun X hXT ).sUnion_eq] at h1
-    simp only [mem_sUnion] at h1
-    obtain ⟨X', hX', heX' ⟩ := h1
-    refine ⟨ X', ⟨⟨X, ⟨hXT, hX'⟩ ⟩, heX'⟩ ⟩
-  intro F hF
-  simp only [ mem_iUnion] at hF
-  obtain ⟨X, hXT, hF⟩ := hF
-  exact hP' M X F (LE.le.subset ((hfun X hXT).subset_ground hF ) ) ((hfun X hXT).pProp F hF)
-
-
-lemma IsCover.cover_typset {P' : Matroid α → Set α → Prop} (hP' : IsMRProp P' )
-    (hcover : M.IsCover P T )
+lemma IsCover.cover_typset {E : Set α}
+    (hcover : T.IsCover E P )
     (f : T → Set (Set α) )
-    (hfun : ∀ X : T, (M ↾ X.1).IsCover P' (f X)) :
-    M.IsCover P' (⋃ X : T, f X ):= by
+    (hfun : ∀ X : T, (f X).IsCover X.1 P' ) :
+    (⋃ X : T, f X ).IsCover E P' := by
   refine ⟨ ?_, ?_ ⟩
   · rw[←hcover.sUnion_eq]
     refine ext ?_
@@ -173,110 +76,178 @@ lemma IsCover.cover_typset {P' : Matroid α → Set α → Prop} (hP' : IsMRProp
       simp only [iUnion_coe_set, mem_sUnion, mem_iUnion] at he
       obtain ⟨T', ⟨ X, ⟨hX, hT'X ⟩ ⟩, hee ⟩ := he
       simp only [mem_sUnion]
-      refine ⟨X, ⟨hX, (mem_of_subset_of_mem (((hfun ⟨X, hX⟩ ).subset_ground hT'X)) hee ) ⟩⟩
+      refine ⟨X, ⟨hX, (mem_of_subset_of_mem (((hfun ⟨X, hX⟩ ).subset hT'X)) hee ) ⟩⟩
     intro he
     simp only [mem_sUnion] at he
     obtain ⟨X, hXT, heX⟩ := he
     simp only [iUnion_coe_set, mem_sUnion, mem_iUnion]
-    have h1 : e ∈ (M ↾ ↑X).E := by exact mem_of_subset_of_mem (fun ⦃a⦄ a_1 ↦ a_1) heX
-    rw[←(hfun ⟨X, hXT⟩ ).sUnion_eq] at h1
-    simp only [mem_sUnion] at h1
-    obtain ⟨X', hX', heX' ⟩ := h1
+    --have h1 : e ∈ ↑X := by exact mem_of_subset_of_mem (fun ⦃a⦄ a_1 ↦ a_1) heX
+    have h1 := (hfun ⟨X, hXT⟩ ).sUnion_eq
+    simp only at h1
+    rw[←h1] at heX
+    simp only [mem_sUnion] at heX
+    obtain ⟨X', hX', heX' ⟩ := heX
     refine ⟨ X', ⟨⟨X, ⟨hXT, hX'⟩ ⟩, heX'⟩ ⟩
   intro F hF
   simp only [iUnion_coe_set, mem_iUnion] at hF
   obtain ⟨X, hXT, hF⟩ := hF
-  exact hP' M X F (LE.le.subset ((hfun ⟨X, hXT⟩).subset_ground hF ) ) ((hfun ⟨X, hXT⟩).pProp F hF)
+  exact (hfun ⟨X, hXT⟩).pProp F hF
+  --exact hP' X F (LE.le.subset ((hfun ⟨X, hXT⟩).subset_ground hF ) ) ((hfun ⟨X, hXT⟩).pProp F hF)
 
-lemma coverNumber_cover_of_covers {P' : Matroid α → Set α → Prop} (hcover : M.IsCover P T)
-    (hP' : IsMRProp P') :
-    M.coverNumber P' ≤ ∑' X : T, (M ↾ X.1).coverNumber P' := by
-  obtain (h0 | h1) := exists_or_forall_not (fun X : T ↦ (M ↾ X).coverNumber P' = ⊤)
+lemma IsCover.cover_fun {P' :  Set α → Prop}
+    (hcover : T.IsCover Y P )
+    (f : Set α → Set (Set α) )
+    (hfun : ∀ X ∈ T, (f X).IsCover X P' ) :
+    ( ⋃ X ∈ T, f X ).IsCover Y P' := by
+  refine ⟨ ?_, ?_ ⟩
+  · rw[←hcover.sUnion_eq]
+    refine ext ?_
+    intro e
+    refine ⟨ ?_, ?_ ⟩
+    · intro he
+      simp only [ mem_sUnion, mem_iUnion] at he
+      obtain ⟨T', ⟨ X, ⟨hX, hT'X ⟩ ⟩, hee ⟩ := he
+      simp only [mem_sUnion]
+      refine ⟨ X ,⟨ hX , mem_of_subset_of_mem ((hfun X hX).subset hT'X ) hee  ⟩ ⟩
+    intro he
+    simp only [mem_sUnion] at he
+    obtain ⟨X, hXT, heX⟩ := he
+    simp only [mem_sUnion, mem_iUnion]
+    --have h1 : e ∈ (M ↾ ↑X).E := by exact mem_of_subset_of_mem (fun ⦃a⦄ a_1 ↦ a_1) heX
+    have h1 := (hfun X hXT ).sUnion_eq
+    rw[←(hfun X hXT ).sUnion_eq] at heX
+    simp only [mem_sUnion] at heX
+    obtain ⟨X', hX', heX' ⟩ := heX
+    refine ⟨ X', ⟨⟨X, ⟨hXT, hX'⟩ ⟩, heX'⟩ ⟩
+  intro F hF
+  simp only [ mem_iUnion] at hF
+  obtain ⟨X, hXT, hF⟩ := hF
+  exact (hfun X hXT).pProp F hF
+  --exact hP' M X F (LE.le.subset ((hfun X hXT).subset_ground hF ) ) ((hfun X hXT).pProp F hF)
+
+lemma IsCover.mono_prop (h : T.IsCover Y P ) (hPP' : ∀ X ∈ T, P X → P' X) : T.IsCover Y P' :=
+  (T.isCover_iff Y P').2 ⟨h.sUnion_eq, fun F hF ↦ hPP' F hF (h.pProp F hF)⟩
+
+lemma IsCover_emptyset_iff (P : Set α → Prop) : IsCover ∅ Y P ↔ ¬Y.Nonempty := by
+  refine ⟨?_, ?_ ⟩
+  · intro h
+    rw [ not_nonempty_iff_eq_empty, ←sUnion_empty, h.sUnion_eq.symm ]
+  intro h
+  rw [ not_nonempty_iff_eq_empty, ←sUnion_empty] at h
+  refine ⟨h.symm, by grind ⟩
+
+lemma Set.IsCover.contract (h : T.IsCover Y P)
+    (hXN : Y.Nonempty)
+    (hPP' : ∀ F : Set α, P F → P' ( F ∪ X) ) :
+    ((· ∪ X) '' T).IsCover (Y ∪ X) P' := by
+  suffices hi : ∀ F ∈ T, P F by
+    simp only [isCover_iff, sUnion_image, mem_image, forall_exists_index, and_imp,
+      forall_apply_eq_imp_iff₂, ← biUnion_distrib_union _ (h.nonempty hXN), ← sUnion_eq_biUnion,
+      h.sUnion_eq, true_and  ]
+      --  ← biUnion_distrib_union _ h.nonempty, ← sUnion_eq_biUnion,
+      -- h.sUnion_eq, contract_ground, diff_union_self, union_eq_left, hX, true_and ]
+    exact fun F hFT ↦ (((fun a ↦ (hPP' F (hi F hFT))) ∘ T) X )
+  exact fun F hFT ↦ h.pProp F hFT
+
+lemma Set.IsCover.mono_set (h : T.IsCover X P ) (hX : Y ⊆ X)
+    (hp : ∀ Z, P Z → P (Z ∩ Y) )
+    : ((· ∩ Y) '' T).IsCover Y P := by
+  refine ⟨?_, ?_ ⟩
+  · simp only [sUnion_image]
+    apply subset_antisymm (iUnion₂_subset_iff.mpr (fun i j ↦ inter_subset_right) )
+    intro y hY
+    have hy : y ∈ X := by exact mem_of_subset_of_mem hX hY
+    rw [←h.sUnion_eq] at hy
+    obtain ⟨T', hT', hT'y ⟩ := hy
+    exact mem_biUnion hT' (mem_inter hT'y hY)
+  intro F hF
+  obtain ⟨Z, hZ, rfl⟩ := hF
+  simp only
+  exact hp Z (h.pProp Z hZ)
+
+end General
+
+section Number
+
+noncomputable def Set.coverNumber (X : Set α) (P : Set α → Prop) : ℕ∞ :=
+  ⨅ (T : Set (Set α)) (_ : T.IsCover X P), T.encard
+
+lemma coverNumber_mono (X : Set α) {P Q : Set α → Prop} (hPQ : ∀ Y ⊆ X, P Y → Q Y) :
+    X.coverNumber Q ≤ X.coverNumber P := by
+  simp only [coverNumber, le_iInf_iff]
+  refine fun T hT ↦ iInf₂_le T ⟨hT.1, fun F hF ↦ hPQ _ ?_ (hT.2 F hF)⟩
+  have := hT.sUnion_eq
+  grind
+
+lemma Set.IsCover.coverNumber_le {T : Set (Set α)} (h : T.IsCover X P ) :
+    X.coverNumber P ≤ T.encard := by
+  simp only [coverNumber, ]
+  exact biInf_le encard h
+
+lemma exists_mincover_NE {P : Set α → Prop}
+    (hn : {T | IsCover T X P }.Nonempty) :
+    ∃ T, IsCover T X P ∧ T.encard = X.coverNumber P := by
+  simp only [coverNumber]
+  simp_rw [iInf_subtype']
+  have := hn.to_subtype
+  obtain ⟨T, hT ⟩ := ENat.exists_eq_iInf (f := fun (T : {T : Set (Set α) | T.IsCover X P}) ↦ T.1.encard)
+  refine ⟨T.1, ⟨T.2, hT ⟩ ⟩
+  -- have := ENat.exists_eq_iInf (f := fun (hT : T.IsCover X P) ↦ T.encard)
+
+lemma exists_min_cover (hP : X.hasCover_with P) :
+    ∃ T, IsCover T X P ∧ T.encard = X.coverNumber P := by
+  exact exists_mincover_NE hP
+
+lemma Set.exists_cover (X : Set α ) (P : Set α → Prop) :
+    X.coverNumber P = ⊤ ∨ ∃ T, IsCover T X P ∧ T.encard = X.coverNumber P := by
+  obtain h0 | h := {T | IsCover T X P }.eq_empty_or_nonempty
+  · left
+    simp only [coverNumber]
+    simp_rw [iInf_subtype']
+    simp only [iInf_eq_top, Subtype.forall]
+    intro T hT
+    by_contra
+    exact Ne.elim (ne_of_mem_of_not_mem' hT fun a ↦ a ) h0
+  right
+  exact exists_min_cover h
+
+lemma coverNumber_positive (hX : X.Nonempty) (P : Set α → Prop) :
+    1 ≤ X.coverNumber P := by
+  by_contra hc
+  have h1 := ENat.lt_one_iff_eq_zero.mp (Std.not_le.mp hc)
+  obtain ht | ⟨T, hT, hTe ⟩ := X.exists_cover P
+  · rw [h1] at ht
+    simp only [ENat.zero_ne_top] at ht
+  have : T.Nonempty := hT.nonempty hX
+  grind
+
+lemma coverNumber_cover_of_covers {P' : Set α → Prop} (hcover : T.IsCover Y P ) :
+    Y.coverNumber P' ≤ ∑' X : T, (X.1).coverNumber P' := by
+  obtain (h0 | h1) := exists_or_forall_not (fun X : T ↦ coverNumber X P' = ⊤)
   · simp [ENat.tsum_eq_top_of_eq_top h0]
-  have hf : ∀ X : T, ∃ XT, (M ↾ X.1).IsCover P' XT ∧
-    XT.encard = (M ↾ X.1).coverNumber P' := by
+  have hf : ∀ X : T, ∃ XT : Set (Set α), XT.IsCover (X.1) P' ∧
+    XT.encard = (X.1).coverNumber P' := by
     intro X
-    obtain (h | ⟨XT, hXres, hencard⟩) := (M ↾ X).exists_cover P'
+    obtain (h | ⟨XT, hXres, hencard⟩) := (X.1).exists_cover P'
     · simp [h1 _ h]
     exact ⟨XT, hXres, hencard⟩
   choose f hfunco hfunca using hf
-  have hcover := IsCover.cover_typset hP' hcover f hfunco
+  have hcover := IsCover.cover_typset hcover f hfunco
   grw [hcover.coverNumber_le, ENat.encard_iUnion_le_tsum_encard, tsum_congr hfunca]
 
-lemma coverNumber_cover_of_covers_bound {P' : Matroid α → Set α → Prop} {k : ℕ∞}
-    (hcover : M.IsCover P T) (hP' : IsMRProp P')
-    (hflat : ∀ F, P M F → (M ↾ F).coverNumber P' ≤ k) :
-    M.coverNumber P' ≤ (T.encard) * k := by
+
+lemma coverNumber_cover_of_covers_bound {P' : Set α → Prop} {k : ℕ∞}
+    (hcover : T.IsCover Y P)
+    (hflat : ∀ F, P F → F.coverNumber P' ≤ k) :
+    Y.coverNumber P' ≤ (T.encard) * k := by
   grw [coverNumber_cover_of_covers hcover, ENat.tsum_le_tsum (g := fun _ ↦ k),
     ENat.tsum_subtype_const, mul_comm]
   intro F
   simp [hflat _ <| hcover.pProp F F.2 ]
-  exact hP'
+  --exact hP'
 
-
---P is minor preserved wrt f if
-def MRProp (α) (P : Matroid α → Set α → Prop) (f : Set α → Matroid α → Set α → Prop ) : Prop :=
-    ∀ M : Matroid α, ∀ Y X : Set α,
-    ∃ (Q : Matroid α → Set α → Prop) , (P (M ／ Y) X → Q M X ∧ Q M X = f Y M X)
-
---Help
-lemma RankIsMRProp (α) {k : ℕ∞} : MRProp (α)
-    (fun M X ↦ M.eRk X ≤ k) (fun Y M X ↦ M.eRk (X ∪ Y) ≤ M.eRk Y + k ) := by
-  intro M Y X
-  use (fun N Z ↦ M.eRk (X ∪ Y) ≤ M.eRk Y + k )
-  simp only [and_true]
-
-  sorry
-
--- --Minor preserved under f
--- --(f : Set α → Matroid α → (Set α → Prop))
--- def IsMUProp (P : Matroid α → Set α → Prop) (X : Set α ) (P' : Matroid α → Set α → Prop): Prop :=
---     --∀ X : Set α,
---     --∃ P' : Matroid α → Set α → Prop,
---     ∀ M : Matroid α,
---     ∀ Y : Set α, P (M ／ X) Y → P' M Y
-
---P ' = k + M.eRk X for rank
-lemma IsCover.contract (h : (M ／ X).IsCover P T)
-    (hX : X ⊆ M.E) (hXN : (M ／ X).Nonempty)
-    (hPP' : ∀ Y : Set α, P (M ／ X) Y → P' M ( Y ∪ X) ) :
-    M.IsCover P' ((· ∪ X) '' T) := by
-  suffices hi : ∀ F ∈ T, P (M ／ X) F by
-    simp only [isCover_iff, sUnion_image, mem_image, forall_exists_index, and_imp,
-      forall_apply_eq_imp_iff₂, ← biUnion_distrib_union _ h.nonempty, ← sUnion_eq_biUnion,
-      h.sUnion_eq, contract_ground, diff_union_self, union_eq_left, hX, true_and ]
-    exact fun F hFT ↦ (((fun a ↦ (hPP' F (hi F hFT))) ∘ T) X )
-  exact fun F hFT ↦ h.pProp F hFT
-
-
---Close under closure
-def IsCCProp (α) (P : Matroid α → Set α → Prop) : Prop :=
-    ∀ M : Matroid α, ∀ F : Set α, P M F → P M (M.closure F)
-
-lemma IsCover.isCover_closure (h : M.IsCover P T) (hP : IsCCProp α P) :
-    M.IsCover P (M.closure '' T) := by
-  simp only [isCover_iff, sUnion_image, subset_antisymm_iff (b := M.E), iUnion_subset_iff,
-    M.closure_subset_ground, implies_true, true_and, mem_image, forall_exists_index, and_imp,
-    forall_apply_eq_imp_iff₂]
-  grw [h.sUnion_eq.symm.subset, sUnion_eq_biUnion]
-  refine  ⟨biUnion_mono rfl.subset fun X hX ↦ M.subset_closure X (h.subset_ground hX),
-  fun F hF ↦ (hP M F (h.pProp F hF)) ⟩
-
---Singleton section
--- noncomputable def SetsingletonEmbedding ( A : Set α ) : Function.Embedding
---     {X : Set α // ∃ e ∈ A, {e} = X} {e // e ∈ A} :=
--- { toFun := fun x => ⟨Classical.choose x.2, (Classical.choose_spec x.2).1 ⟩
---   inj' := by
---     intro x y hxy
---     simp only [Subtype.mk.injEq] at hxy
---     have heq : x.1 = y.1 := by
---       rw [←(Classical.choose_spec x.2).2, ←(Classical.choose_spec y.2).2]
---       exact singleton_eq_singleton_iff.mpr hxy
---     exact Subtype.ext heq
---     }
-
-lemma IsCover_singleton_Prop (hP : ∀ e ∈ M.E, P M (singleton e)) :
-    M.IsCover P (singleton '' M.E) := by
+lemma IsCover_singleton_Prop (hP : ∀ e ∈ X, P (singleton e)) :
+    (singleton '' X).IsCover X P  := by
   refine ⟨ ?_, ?_ ⟩
   · refine Eq.symm (ext ?_)
     intro x
@@ -292,29 +263,16 @@ lemma IsCover_singleton_Prop (hP : ∀ e ∈ M.E, P M (singleton e)) :
   rw[←heF]
   exact hP e heE
 
-
-lemma IsCover_singleton_le (hP : ∀ e ∈ M.E, P M (singleton e)) :
-    M.coverNumber P ≤ M.E.encard := by
+lemma IsCover_singleton_le (hP : ∀ e ∈ X, P (singleton e)) :
+    X.coverNumber P ≤ X.encard := by
   grw [(IsCover_singleton_Prop hP).coverNumber_le ]
-  set Sing : Set (Set α ) := { singleton e | e ∈ M.E} with hs
-  exact encard_image_le singleton M.E
+  set Sing : Set (Set α ) := { singleton e | e ∈ X} with hs
+  exact encard_image_le singleton X
 
-
-lemma IsCover.mono_prop (h : M.IsCover P T) (hPP' : ∀ X ∈ T, P M X → P' M X) : M.IsCover P' T :=
-  (M.isCover_iff P' T).2 ⟨h.sUnion_eq, fun F hF ↦ hPP' F hF (h.pProp F hF)⟩
-
-lemma IsCover_emptyset_iff (P : Matroid α → Set α → Prop) : M.IsCover P ∅ ↔ ¬M.Nonempty := by
+lemma coverNumber_zero_iff (P : Set α → Prop) : X.coverNumber P = 0 ↔ IsCover ∅ X P := by
   refine ⟨?_, ?_ ⟩
   · intro h
-    rw [ ←Matroid.ground_nonempty_iff, not_nonempty_iff_eq_empty, ←sUnion_empty, h.sUnion_eq.symm ]
-  intro h
-  rw [ ←Matroid.ground_nonempty_iff, not_nonempty_iff_eq_empty, ←sUnion_empty] at h
-  refine ⟨h.symm, by grind ⟩
-
-lemma coverNumber_zero_iff (P : Matroid α → Set α → Prop) : M.coverNumber P = 0 ↔ M.IsCover P ∅ := by
-  refine ⟨?_, ?_ ⟩
-  · intro h
-    obtain ht | ⟨T, hT, hTe ⟩ := exists_cover M P
+    obtain ht | ⟨T, hT, hTe ⟩ := exists_cover X P
     · by_contra
       rw[ht] at h
       simp only [ENat.top_ne_zero] at h
@@ -325,133 +283,256 @@ lemma coverNumber_zero_iff (P : Matroid α → Set α → Prop) : M.coverNumber 
   simp only [encard_empty, nonpos_iff_eq_zero] at this
   grind
 
-lemma coverNumber_le_coverNumber (P Q : Matroid α → Set α → Prop) (M : Matroid α)
-    (hPQ : ∀ X ⊆ M.E, P M X → Q M X) : M.coverNumber Q ≤ M.coverNumber P := by
+lemma coverNumber_le_coverNumber (P Q : Set α → Prop) (X : Set α )
+    (hPQ : ∀ Y ⊆ X, P Y → Q Y) : X.coverNumber Q ≤ X.coverNumber P := by
+  obtain ht | ⟨T, hT, hTe ⟩ := exists_cover X P
+  · rw [ht]
+    simp only [le_top]
+  rw [←hTe]
+  exact IsCover.coverNumber_le ⟨hT.sUnion_eq, fun F hF ↦ hPQ F (hT.subset hF) (hT.pProp F hF) ⟩
+
+lemma coverNumber_congr (P Q : Set α → Prop)
+    (hPQ : ∀ (Y : Set α), Y ⊆ X → (P Y ↔ Q Y)) :
+    X.coverNumber P = X.coverNumber Q := by
   sorry
 
-lemma coverNumber_congr (P Q : Matroid α → Set α → Prop)
-    (hPQ : ∀ (M : Matroid α) (X : Set α), X ⊆ M.E → (P M X ↔ Q M X)) (M : Matroid α) :
-    M.coverNumber P = M.coverNumber Q := by
-  sorry
 
-lemma coverNumber_mono_prop (P : Matroid α → Set α → Prop) {M N : Matroid α} (hMN : M.E = N.E)
-    (hMP : ∀ X ⊆ M.E, P N X → P M X) : M.coverNumber P ≤ N.coverNumber P := by
+end Number
 
---   simp only [coverNumber, le_sInf_iff, mem_image, mem_setOf_eq, forall_exists_index, and_imp,
+
+
+-- def IsCCProp (α) (P : Matroid α → Set α → Prop) : Prop :=
+--     ∀ M : Matroid α, ∀ F : Set α, P M F → P M (M.closure F)
+
+-- lemma IsCover.isCover_closure (h : M.IsCover P T) (hP : IsCCProp α P) :
+--     M.IsCover P (M.closure '' T) := by
+--   simp only [isCover_iff, sUnion_image, subset_antisymm_iff (b := M.E), iUnion_subset_iff,
+--     M.closure_subset_ground, implies_true, true_and, mem_image, forall_exists_index, and_imp,
 --     forall_apply_eq_imp_iff₂]
---   refine fun C hC ↦ sInf_le ?_
---   simp only [mem_image, mem_setOf_eq]
---   refine ⟨C, ?_, rfl⟩
---   have := hC.mono_prop (P' := P)
+--   grw [h.sUnion_eq.symm.subset, sUnion_eq_biUnion]
+--   refine  ⟨biUnion_mono rfl.subset fun X hX ↦ M.subset_closure X (h.subset_ground hX),
+--   fun F hF ↦ (hP M F (h.pProp F hF)) ⟩
+namespace Matroid
+section Matroid
+
+def IsCCProp (P : Matroid α → Set α → Prop) : Prop :=
+    ∀ M : Matroid α, ∀ F : Set α, P M F → P M (M.closure F)
+
+lemma Set.IsCover.isCover_closure {P : Matroid α → Set α → Prop} {M :Matroid α }
+    (h : T.IsCover X (P M)) (hP : IsCCProp P) (hXc : M.IsFlat X) (hX : X ⊆ M.E) :
+    (M.closure '' T).IsCover X (P M) := by
+  simp only [isCover_iff, sUnion_image, mem_image, forall_exists_index, and_imp,
+    forall_apply_eq_imp_iff₂, subset_antisymm_iff (b := X), iUnion_subset_iff, mem_image,
+    forall_exists_index, and_imp, forall_apply_eq_imp_iff₂]
+  nth_rw 1 [←M.isFlat_iff_closure_self.1 hXc ]
+  refine ⟨⟨fun T' hT' ↦ closure_subset_closure_of_subset_closure
+    (by simp only [M.isFlat_iff_closure_self.1 hXc,IsCover.subset h hT' ]) , ?_ ⟩,
+    fun F hF ↦ (hP M F (h.pProp F hF)) ⟩
+  · grw [h.sUnion_eq.symm.subset, sUnion_eq_biUnion]
+    refine biUnion_mono rfl.subset fun Z hZ ↦ (subset_closure_iff_forall_subset_isFlat Z
+      (LE.le.subset fun ⦃a⦄ a_1 ↦ hX ((IsCover.subset h hZ ) a_1) )).mpr fun F a a_1 ↦ a_1
+
+-- lemma Set.IsCover.isCover_closure {P : Matroid α → Set α → Prop} {M :Matroid α }
+--     (h : T.IsCover X (P M)) (hP : IsCCProp P) :
+--     (M.closure '' T).IsCover (M.closure X) (P M) := by
+--   simp only [isCover_iff, sUnion_image, mem_image, forall_exists_index, and_imp,
+--     forall_apply_eq_imp_iff₂, mem_image,
+--     forall_exists_index, and_imp, forall_apply_eq_imp_iff₂]
+--   refine ⟨ ?_, ?_ ⟩
+--   · apply subset_antisymm_iff.2 ?_
+--     simp only [iUnion_subset_iff]
+--     refine ⟨fun T' hT' ↦ (closure_subset_closure M (h.subset hT')), ?_ ⟩
+--     rw [←h.sUnion_eq]
+
+--     sorry
+--   sorry
 
 
-end General
+-- lemma coverNumber_mono_prop (P : Set α → Prop) {M N : Matroid α} (hMN : M.E = N.E)
+--     (hMP : ∀ X ⊆ M.E, P N X → P M X) : M.coverNumber P ≤ N.coverNumber P := by
+
+
+end Matroid
 
 section Rank
 
--- lemma RankPropIsMUProp {k : ℕ∞} : IsMUProp (RankProp α k) (fun M X Y ↦ (M.eRk Y ≤ k + M.eRk X)) := by
---     --use fun M X Y ↦ (M.eRk Y ≤ k + M.eRk X)
---     intro M X Y hXY
---     unfold RankProp at hXY
---     sorry
+def IsRankCover (M : Matroid α) (T : Set (Set α)) (X : Set α) (k : ℕ∞) :=
+    T.IsCover X (fun A ↦ M.eRk A ≤ k)
 
-def IsRankCover (M : Matroid α) (k : ℕ∞) (T : Set (Set α )) : Prop :=
-    M.IsCover (fun M X ↦ M.eRk X ≤ k) T
+lemma IsRankCover.contract (h : (M ／ X).IsRankCover T Y k )
+    (hXN : Y.Nonempty) :
+    M.IsRankCover ((· ∪ X) '' T) (Y ∪ X) (k + M.eRk X)  := by
+  unfold IsRankCover
+  unfold IsRankCover at h
+  apply IsCover.contract h hXN
+  intro F hF
+  rw [← @eRelRk_add_eRk_eq, eRelRk_eq_eRk_contract]
+  exact add_le_add_left hF (M.eRk X)
 
-lemma IsRankCover_iff_IsCover (M : Matroid α) (k : ℕ∞) (T : Set (Set α )) :
-    M.IsRankCover k T ↔ M.IsCover (fun M X ↦ M.eRk X ≤ k) T := Iff.rfl
+lemma IsRankCover_iff_IsCover {M : Matroid α} {T : Set (Set α)} {X : Set α} {k : ℕ∞} :
+    M.IsRankCover T X k ↔ T.IsCover X (fun A ↦ M.eRk A ≤ k) := Iff.rfl
 
-lemma IsRankCover_iff (M : Matroid α) (k : ℕ∞) (T : Set (Set α )) :
-    M.IsRankCover k T ↔ ⋃₀ T = M.E ∧ (∀ F ∈ T, M.eRk F ≤ k) := by
-  sorry
   --Mathieu
+lemma IsRankCover_iff (M : Matroid α) (T : Set (Set α)) (X : Set α) (k : ℕ∞) :
+    M.IsRankCover T X k ↔ ⋃₀ T = X ∧ (∀ F ∈ T, M.eRk F ≤ k) := by
+  sorry
 
-lemma IsRankCover_isCover_closure (hcov : M.IsRankCover k T) :
-    M.IsRankCover k (M.closure '' T) := by
-  apply hcov.isCover_closure (fun M F hF ↦ ?_)
+lemma IsRankCover_iff_restriction (hX : X ⊆ M.E) :
+    M.IsRankCover T X k ↔ (M ↾ X).IsRankCover T (M ↾ X).E k := by
+  sorry
+
+lemma IsRankCover.subset (h : M.IsRankCover T X k) (hY : Y ∈ T) : Y ⊆ X :=
+  (IsRankCover_iff_IsCover.1 h ).subset hY
+
+lemma IsRankCover.subset_ground (h : M.IsRankCover T X k) (hY : Y ∈ T)
+    (hX : X ⊆ M.E := by aesop_mat) : Y ⊆ M.E :=
+  LE.le.subset fun ⦃a⦄ a_1 ↦ hX (((IsRankCover_iff_IsCover.1 h ).subset hY ) a_1)
+
+lemma IsRankCover.mono_set (hcov : M.IsRankCover T X k) (hX : Y ⊆ X) :
+    M.IsRankCover ((· ∩ Y) '' T) Y k := by
+  rw [IsRankCover_iff_IsCover]
+  rw [IsRankCover_iff_IsCover]  at hcov
+  apply hcov.mono_set hX
+  intro F hF
+  grw [eRk_subset_le M inter_subset_left, hF]
+
+lemma IsRankCover_isCover_closure (hcov : M.IsRankCover T X k) (hX : M.IsFlat X) :
+    M.IsRankCover (M.closure '' T) X k := by
+  rw [IsRankCover_iff_IsCover]
+  rw [IsRankCover_iff_IsCover]  at hcov
+  apply Set.IsCover.isCover_closure hcov (fun M F hF ↦ ?_) hX (hX.subset_ground)
   rwa [(eRk_closure_eq M F) ]
 
-lemma IsRankCover.mono_k {k' : ℕ∞} (hcov : M.IsRankCover k T) (hkk' : k ≤ k') :
-    M.IsRankCover k' T := by
+-- lemma IsRankCover_isCover_closure (hcov : M.IsRankCover T X k) :
+--     M.IsRankCover (M.closure '' T) (M.closure X) k := by
+
+--   sorry
+
+lemma IsRankCover.mono_k {k' : ℕ∞} (hcov : M.IsRankCover T X k) (hkk' : k ≤ k') :
+    M.IsRankCover T X k' := by
   refine ⟨ hcov.sUnion_eq, fun F hF ↦
     Std.IsPreorder.le_trans (M.eRk F) k k' (hcov.pProp F hF ) hkk' ⟩
 
-lemma IsRankCover_RankPos : M.hasCover_with (fun M X ↦ M.eRk X ≤ 0) ↔ ¬ M.RankPos := by
+lemma IsRankCover.one_le (h : M.IsRankCover T X k) (hX : X.Nonempty) :
+    1 ≤ T.encard := IsCover.one_le h hX
+
+lemma IsRankCover_Zero (X : Set α) (hX : X ⊆ M.E := by aesop_mat) :
+    X.hasCover_with (fun A ↦ M.eRk A ≤ 0) ↔ X ⊆ M.loops := by
   refine ⟨ ?_, ?_ ⟩
-  · intro h
-    refine M.not_rankPos_iff.2 (Matroid.eq_loopyOn_iff_loops.mpr
-      ⟨Eq.symm (Subset.antisymm ?_ (loops_subset_ground M )) , by simp only ⟩   )
-    intro e he
-    obtain ⟨ T, hT ⟩ := h
-    rw[←hT.sUnion_eq ] at he
-    obtain ⟨ X, hXt, heX ⟩ := he
-    exact isLoop_iff.mp (((Matroid.eRk_eq_zero_iff (IsCover.subset_ground hT hXt  )).1
-      (nonpos_iff_eq_zero.mp (hT.pProp X hXt ))) heX)
+  · intro h e he
+    obtain ⟨ T', hT' ⟩ := h
+    rw[←hT'.sUnion_eq ] at he
+    obtain ⟨ Y, hYt, heY ⟩ := he
+    apply isLoop_iff.mp
+    exact isLoop_iff.mp (((Matroid.eRk_eq_zero_iff ((IsRankCover_iff_IsCover.2 hT').subset_ground hYt  )).1
+      (nonpos_iff_eq_zero.mp (hT'.pProp Y hYt ))) heY)
   intro h
-  refine ⟨ (singleton '' M.E), IsCover_singleton_Prop ?_ ⟩
+  refine ⟨ (singleton '' X), IsCover_singleton_Prop ?_ ⟩
   intro e he
   simp only [nonpos_iff_eq_zero]
   refine IsLoop.eRk_eq ?_
-  rw [M.not_rankPos_iff.1 h]
-  exact loopyOn_isLoop_iff.mpr he
+  exact isLoop_iff.mpr (h he)
 
-lemma IsRankCover_two [M.Nonempty] (hcov : M.IsRankCover k T) (hk : k < M.eRank ) :
+lemma IsRankCover_RankPos :
+    (M.E).hasCover_with (fun A ↦ M.eRk A ≤ 0) ↔ ¬ M.RankPos := by
+  refine ⟨fun h ↦ (M.not_rankPos_iff.2 (Matroid.eq_loopyOn_iff_loops.mpr
+    ⟨Eq.symm (Subset.antisymm ((IsRankCover_Zero M.E).1 h ) (loops_subset_ground M )),
+    by simp only ⟩)) , fun h ↦ (IsRankCover_Zero M.E fun ⦃a⦄ a_1 ↦ a_1).mpr
+    (subset_of_subset_of_eq (fun ⦃a⦄ a_1 ↦ a_1) (Eq.symm (Matroid.eq_loopyOn_iff_loops.1
+    (M.not_rankPos_iff.1 h )).1)) ⟩
+
+lemma IsRankCover_two (hcov : M.IsRankCover T X k) (hk : k < M.eRk X ) :
     2 ≤ T.encard := by
   by_contra hc
   simp only [not_le] at hc
+  have hXne : X.Nonempty := by
+    by_contra hc
+    simp only [Set.nonempty_iff_ne_empty, ne_eq, Decidable.not_not] at hc
+    rw [hc] at hk
+    have : 0 ≤ k := by exact ENat.zero_le
+    have hg : 0 < M.eRk ∅ := by grind
+    rw [eRk_empty M] at hg
+    exact (lt_self_iff_false 0).mp hg
   have hle : T.encard ≤ 1 := Order.le_of_lt_succ hc
-  have h1 := ((IsRankCover_iff_IsCover M k T).1 hcov).one_le
+  have h1 := hcov.one_le
   have h1 : T.encard = 1 := by grind
-  obtain ⟨X, hX ⟩ := Set.encard_eq_one.1 h1
-  have h2 := ((IsRankCover_iff_IsCover M k T).1 hcov).sUnion_eq
-  rw [hX] at h2
+  obtain ⟨X', hX' ⟩ := Set.encard_eq_one.1 h1
+  have h2 := ((IsRankCover_iff_IsCover).1 hcov).sUnion_eq
+  rw [hX'] at h2
   simp only [sUnion_singleton] at h2
-  have hXT : X ∈ T := by
-    rw[ hX ]
-    exact mem_singleton X
-  have hf := ((IsRankCover_iff_IsCover M k T).1 hcov).pProp X hXT
-  rw[ h2, ←eRank_def M  ] at hf
+  have hXT : X' ∈ T := by
+    rw[ hX' ]
+    exact mem_singleton X'
+  have hf := ((IsRankCover_iff_IsCover).1 hcov).pProp X' hXT
+  rw[ h2] at hf
   grind
 
+lemma setOf_point_IsRankCover (M : Matroid α) (X : Set α) [(M ↾ X).RankPos] :
+    M.IsRankCover {P | (M ↾ X).IsPoint P} X 1 := by
+  refine ⟨subset_antisymm (sUnion_subset fun _ ↦ IsPoint.subset_ground) fun e he ↦ ?_, ?_ ⟩
+  · simp only [mem_sUnion, mem_setOf_eq]
+    obtain hl | hnl := (M ↾ X).isLoop_or_isNonloop e
+    · obtain ⟨f, hf⟩ := (M ↾ X).exists_isNonloop
+      exact ⟨_, hf.closure_isPoint, hl.mem_closure _⟩
+    exact ⟨_, hnl.closure_isPoint, mem_closure_of_mem _ (by simp) (by simpa)⟩
+  intro F hF
+  simp only [mem_setOf_eq] at hF
+  have hgs := hF.subset_ground
+  simp only [restrict_ground_eq] at hgs
+  grw [← inter_eq_left.2 (LE.le.subset hgs), ←restrict_eRk_eq', hF.eRk ]
 
-lemma setOf_point_IsRankCover (M : Matroid α) [M.RankPos] : M.IsRankCover 1 {P | M.IsPoint P} := by
-  refine ⟨subset_antisymm (sUnion_subset fun _ ↦ IsPoint.subset_ground) fun e he ↦ ?_,
-    by simp +contextual [mem_setOf_eq, IsPoint] ⟩
-  simp only [mem_sUnion, mem_setOf_eq]
-  obtain hl | hnl := M.isLoop_or_isNonloop e
-  · obtain ⟨f, hf⟩ := M.exists_isNonloop
-    exact ⟨_, hf.closure_isPoint, hl.mem_closure _⟩
-  exact ⟨_, hnl.closure_isPoint, mem_closure_of_mem _ (by simp) (by simpa)⟩
-
-lemma setOf_point_IsCover [hM : M.Loopless] : M.IsRankCover 1 {P | M.IsPoint P} := by
-  obtain ⟨E, rfl⟩ | h := M.eq_loopyOn_or_rankPos'
-  · obtain rfl : E = ∅ := by simpa using hM
+lemma setOf_point_IsCover [hM : (M ↾ X).Loopless] : M.IsRankCover {P | (M ↾ X).IsPoint P} X 1 := by
+  obtain ⟨E, hX⟩ | h := (M ↾ X).eq_loopyOn_or_rankPos'
+  · rw [hX]
+    rw [hX] at hM
+    obtain rfl : E = ∅ := by simpa using hM
     constructor <;> simp [IsPoint]
-  exact M.setOf_point_IsRankCover
+    rw [ ←restrict_ground_eq (M := M) (R := X), hX ]
+    simp only [loopyOn_empty, emptyOn_ground, sUnion_eq_empty, mem_setOf_eq, and_imp, forall_eq,
+      eRk_empty, zero_ne_one, implies_true]
+  exact M.setOf_point_IsRankCover X
 
-lemma IsRankCover_ground (M : Matroid α) : M.IsRankCover M.eRank ({M.E}) := by
-  refine ⟨ by simp, fun F a ↦ eRk_le_eRank M F ⟩
+-- M.eRank ({M.E})
+lemma IsRankCover_ground (M : Matroid α) : M.IsRankCover ({X}) X (M.eRk X) := by
+  refine ⟨ by simp, ?_ ⟩
+  intro F hF
+  simp only [mem_singleton_iff] at hF
+  rw [hF]
 
-lemma IsRankCover.nonempty [M.Nonempty] (h : M.IsRankCover k T) : T.Nonempty := by
+lemma IsRankCover.nonempty (h : M.IsRankCover T X k) (hX : X.Nonempty) : T.Nonempty := by
   rw [nonempty_iff_empty_ne]
   rintro rfl
-  simp [IsRankCover_iff, eq_comm, M.ground_nonempty.ne_empty] at h
+  simp [IsRankCover_iff, eq_comm] at h
+  exact Ne.elim (Set.nonempty_iff_empty_ne.1 hX ) (Eq.symm h)
 
-lemma RankPropCover_exists (hk : 1 ≤ k) : M.hasCover_with (fun M X ↦ M.eRk X ≤ k) := by
-  by_cases hRP : M.RankPos
-  · refine ⟨{P | M.IsPoint P}, (setOf_point_IsRankCover M ).mono_k hk ⟩
-  obtain ⟨ T, hT ⟩ := IsRankCover_RankPos.2 hRP
-  refine ⟨ T, ((IsRankCover_iff_IsCover M 0 T).2 hT).mono_k (ENat.zero_le ) ⟩
+lemma RankPropCover_exists (M : Matroid α) (hk : 1 ≤ k) (hX : X ⊆ M.E) :
+    X.hasCover_with (fun A ↦ M.eRk A ≤ k) := by
+  by_cases hRP : (M ↾ X).RankPos
+  · refine ⟨{P | (M ↾ X).IsPoint P}, IsRankCover_iff_IsCover.1
+      ((M.setOf_point_IsRankCover X ).mono_k hk) ⟩
+  have hXl : X ⊆ M.loops := by
+    rw [not_rankPos_iff, restrict_ground_eq] at hRP
+    refine (eRk_eq_zero_iff hX).mp ?_
+    rw [Eq.symm (eRank_restrict M X), hRP]
+    exact eRank_loopyOn X
+  obtain ⟨ T, hT ⟩ := (IsRankCover_Zero X).2 hXl
+  refine ⟨ T, IsRankCover_iff_IsCover.1 (IsRankCover.mono_k hT (ENat.zero_le))  ⟩
 
-lemma IsCover.delete (hT : M.IsCover (fun M X ↦ M.eRk X ≤ k) T) (D : Set α) :
-    (M ＼ D).IsCover (fun M X ↦ M.eRk X ≤ k) ((fun s ↦ s \ D) '' T) := by
+lemma RankPropCover_exists_min_cover (M : Matroid α) (hk : 1 ≤ k) (hX : X ⊆ M.E) :
+    ∃ T, M.IsRankCover T X k ∧ T.encard = X.coverNumber (fun A ↦ M.eRk A ≤ k) := by
+  simp only [IsRankCover_iff_IsCover]
+  exact exists_min_cover (RankPropCover_exists M hk hX)
+
+lemma IsRankCover.delete (hT : M.IsRankCover T X k) (D : Set α) :
+    M.IsRankCover ((fun s ↦ s \ D) '' T) (X \ D) k := by
+    --(M ＼ D).IsCover (fun M X ↦ M.eRk X ≤ k) ((fun s ↦ s \ D) '' T) := by
   refine ⟨ ?_, ?_ ⟩
   · refine subset_antisymm (sUnion_subset fun K ↦ ?_) fun e he ↦ ?_
     · intro hK
       obtain ⟨ X, hX, h ⟩ := hK
       rw[ ← h]
-      exact diff_subset_diff_left (hT.subset_ground hX )
-    simp only [delete_ground, mem_diff] at he
+      exact diff_subset_diff_left (hT.subset hX )
+    simp only [mem_diff] at he
     rw [←hT.sUnion_eq] at he
     obtain ⟨X, hX, hXe ⟩ := he.1
     have : e ∈ X \ D := mem_diff_of_mem hXe (he.2 )
@@ -459,166 +540,122 @@ lemma IsCover.delete (hT : M.IsCover (fun M X ↦ M.eRk X ≤ k) T) (D : Set α)
   intro F hF
   obtain ⟨ F' ,hF' ,hF2 ⟩ := hF
   rw [←hF2]
-  simp only [delete_eRk_eq', sdiff_idem]
+  --simp only [delete_eRk_eq', sdiff_idem]
   grw [eRk_subset_le M (diff_subset)]
   exact hT.pProp F' hF'
 
---Help
-lemma coverNumber_eRank [M.Nonempty] : M.coverNumber (fun M' X ↦ M'.eRk X ≤ M.eRank) = 1 := by
-  have h2 : 1 ≤ M.coverNumber (fun M' X ↦ M'.eRk X ≤ M.eRank ) :=
-    M.coverNumer_positive (fun M' X ↦ M'.eRk X ≤ M.eRank )
+lemma IsRankcoverNumber_eRank (hX : X.Nonempty) :
+    X.coverNumber (fun A ↦ M.eRk A ≤ (M.eRk X)) = 1 := by
+  have h2 : 1 ≤ X.coverNumber (fun A ↦ M.eRk A ≤ (M.eRk X)) :=
+    coverNumber_positive hX (fun A ↦ M.eRk A ≤ (M.eRk X))
   refine h2.antisymm' ?_
   simpa using (IsRankCover_ground M).coverNumber_le
 
-lemma coverNumber_delete_loop (hne : (M ＼ D).Nonempty) (hk : 1 ≤ k) (hD : D ⊆ M.loops ) :
-    M.coverNumber (fun M X ↦ M.eRk X ≤ k) = (M ＼ D).coverNumber (fun M X ↦ M.eRk X ≤ k) := by
-  obtain ⟨T, hT, hTen ⟩ := exists_min_cover (RankPropCover_exists (M := M) hk )
+--Ask Peter
+lemma IsRankcoverNumber_delete_loop (hne : (X \ D).Nonempty) (hk : 1 ≤ k) (hD : D ⊆ M.loops )
+    (hX : X ⊆ M.E) :
+    X.coverNumber (fun A ↦ M.eRk A ≤ k) = (X \ D).coverNumber (fun A ↦ M.eRk A ≤ k) := by
+  obtain ⟨T, hT, hTen ⟩ := exists_min_cover (RankPropCover_exists (M := M) hk hX)
+  rw [←IsRankCover_iff_IsCover] at hT
   have h1 := (hT.delete D ).coverNumber_le
   grw[encard_image_le (fun s ↦ s \ D) T, hTen ] at h1
-  -- have hkD : (M ＼ D).RankPos := by
-  --   have hh : (M ＼ M.loops).RankPos := Delete_loops_RankPos
-  --   rw [Matroid.rankPos_iff ] at hh
-  --   simp only [delete_isBase_iff] at hh
-  --   refine { empty_not_isBase := ?_ }
-  --   by_contra hc
-  --   exact Ne.elim (fun a ↦ hh ((((Matroid.IsBasis.isBasis_subset (isBasis_ground_iff.mpr hc )
-  --   (empty_subset (M.E \ D) ) (IsLoopEquiv.subset_ground rfl fun ⦃a⦄ a_1 ↦ a_1) ) ).isBasis_subset
-  --     (empty_subset (M.E \ M.loops) ) (diff_subset_diff_right hD ) ).of_delete)) hTen
-  --have : (M ＼ D).Nonempty := rankPos_nonempty
-  obtain ⟨T', hT', hT'en ⟩ := exists_min_cover (RankPropCover_exists (M := (M ＼ D)) hk )
-  have hcov : M.IsCover (fun M X ↦ M.eRk X ≤ k) (M.closure '' T' ) := by
+  have hh : X \ D ⊆ M.E := by
+    simp only [diff_subset_iff, subset_union_of_subset_right hX D ]
+  obtain ⟨T', hT', hT'en ⟩ := exists_min_cover (RankPropCover_exists (M := M) hk hh )
+  have hcov : ( (· ∪ (D ∩ X)) '' T' ).IsCover X (fun A ↦ M.eRk A ≤ k) := by
+  --have hcov : ((M ↾ X).closure '' T' ).IsCover X (fun A ↦ M.eRk A ≤ k) := by
+  --have hcov : M.IsCover (fun M X ↦ M.eRk X ≤ k) (M.closure '' T' ) := by
     refine ⟨ ?_, ?_ ⟩
     · refine subset_antisymm (sUnion_subset fun K ↦ ?_) fun e he ↦ ?_
-      · simp only [mem_image, forall_exists_index, and_imp]
+      · simp only [mem_image, forall_exists_index, and_imp ]
+        intro x hxT' h
+        rw [← h]
+        simp only [union_subset_iff, inter_subset_right, and_true]
+        have := hT'.subset hxT'
         grind
       by_cases heD : e ∈ D
-      · obtain ⟨ X, hX ⟩ := hT'.nonempty
-        have := (IsLoop.mem_closure (hD heD) X )
+      · obtain ⟨ Y, hY ⟩ := hT'.nonempty hne
+        have : e ∈ D ∩ X := by exact mem_inter heD he
         grind
-      have h2 : e ∈ M.E \ D := mem_diff_of_mem he heD
-      rw[←delete_ground,  ←hT'.sUnion_eq  ] at h2
-      obtain ⟨ X, hX, heX ⟩ := h2
-      have := (mem_closure_of_mem' M heX he )
+        -- have hD : D ∩ X ⊆ (M ↾ X).loops := by
+        --   rw [restrict_loops_eq hX ]
+        --   exact inter_subset_inter hD fun ⦃a⦄ a_1 ↦ a_1
+        -- have := (IsLoop.mem_closure (hD (mem_inter heD he )) Y )
+        --have : e ∈
+        --grind
+      have h2 : e ∈ X \ D := mem_diff_of_mem he heD
+      rw[←hT'.sUnion_eq  ] at h2
+      obtain ⟨ Y, hY, heY ⟩ := h2
+      have : e ∈ Y ∪ (D ∩ X) := by exact mem_union_left (D ∩ X) heY
       grind
+      -- have h2 : e ∈ X \ D := mem_diff_of_mem he heD
+      -- --←M.restrict_ground_eq (R := X), ←delete_ground,
+      -- rw[←hT'.sUnion_eq  ] at h2
+      -- obtain ⟨ Y, hY, heY ⟩ := h2
+      -- have := (mem_closure_of_mem' (M ↾ X) heY he )
+      -- grind
     intro F hF
     obtain ⟨F' ,hF', hF2 ⟩ := hF
-    rw[←hF2, eRk_closure_eq M F']
-    have ha := hT'.pProp F' hF'
-    simp only [delete_eRk_eq'] at ha
-    have ha1 : F' \ D = F' := by
-      have := hT'.subset_ground hF'
-      grind
-    rwa [ha1] at ha
-  have h2 := hcov.coverNumber_le
-  grw [encard_image_le M.closure T', hT'en] at h2
-  grind
+    simp only at hF2
+    have : F' ∪ (D ∩ X) ⊆ X := by
+      refine union_subset ?_ (by grind)
+      sorry
+    -- union_subset (LE.le.subset fun ⦃a⦄ a_1 ↦ (diff_subset) ( (hT'.subset hF') a_1)) (inter_subset_right )
+    rw [←hF2, ←restrict_eRk_eq (R := X)]
+    sorry
 
-lemma coverNumber_contract_loop (hne : (M ＼ D).Nonempty) (hk : 1 ≤ k) (hD : D ⊆ M.loops ) :
-    M.coverNumber (fun M X ↦ M.eRk X ≤ k) = (M ／ D).coverNumber (fun M X ↦ M.eRk X ≤ k) := by
-  rw[contract_eq_delete_of_subset_loops hD]
-  exact coverNumber_delete_loop hne hk hD
-
-lemma IsRankCover.contract (h : (M ／ X).IsRankCover k T) (hX : X ⊆ M.E)
-    (hXN : (M ／ X).Nonempty) :
-    M.IsRankCover (k + M.eRk X) ((· ∪ X) '' T) := by
-  suffices ∀ F ∈ T, M.eRk (F ∪ X) ≤ k + M.eRk X by
-    simpa [IsRankCover_iff, ← biUnion_distrib_union _ h.nonempty, ← sUnion_eq_biUnion, h.sUnion_eq, hX]
-  exact fun F hFT ↦ by grw [← h.pProp F hFT, ← eRelRk_eq_eRk_contract, eRelRk_add_eRk_eq]
-
-lemma coverNumber_contract_one {a : ℕ∞} (he : e ∈ M.E) (hel : M.IsNonloop e)
-    (heN : (M／ {e}).Nonempty) :
-    M.coverNumber (fun M X ↦ M.eRk X ≤ (a + 1)) ≤ (M ／ {e}).coverNumber (fun M X ↦ M.eRk X ≤ a)
+    --have := removeLoops_eRank_eq
+    sorry
+    -- intro F hF
+    -- obtain ⟨F' ,hF', hF2 ⟩ := hF
+    -- have : (M ↾ X).closure F' ⊆ X := by
+    --   refine IsFlat.closure_subset_of_subset ?_ ?_
+    --   sorry
+    --   sorry
+    -- rw[←hF2, ←restrict_eRk_eq (R := X),  eRk_closure_eq (M ↾ X) F']
+    -- have ha := hT'.pProp F' hF'
+    -- simp only [delete_eRk_eq'] at ha
+    -- have ha1 : F' \ D = F' := by
+    --   have := hT'.subset_ground hF'
+    --   grind
+    -- rwa [ha1] at ha
+  -- have h2 := hcov.coverNumber_le
+  -- grw [encard_image_le (M ↾ X).closure T', hT'en] at h2
+  -- grind
+  sorry
+lemma IsRankcoverNumber_contract_one {a : ℕ∞} (hel : M.IsNonloop e) (heX : e ∈ X)
+    (hne : (X \ {e}).Nonempty) :
+    X.coverNumber (fun A ↦ M.eRk A ≤ (a + 1)) ≤ (X \ {e}).coverNumber (fun A ↦ (M ／ {e}).eRk A ≤ a)
     := by
-  refine ENat.forall_natCast_le_iff_le.mp ?_
-  intro b hb
-  unfold coverNumber at hb
-  simp only [le_sInf_iff, mem_image, mem_setOf_eq, forall_exists_index, and_imp,
-    forall_apply_eq_imp_iff₂] at hb
-  unfold coverNumber
-  simp only [le_sInf_iff, mem_image, mem_setOf_eq, forall_exists_index, and_imp,
-    forall_apply_eq_imp_iff₂]
-  intro T hT
-  rw[←IsRankCover_iff_IsCover] at hT
-  have h1 := hT.contract (singleton_subset_iff.mpr he ) heN
-  rw[IsNonloop.eRk_eq hel ] at h1
-  have h2 := hb ((· ∪ {e}) '' T) h1
-  grw[encard_image_le (fun x ↦ x ∪ {e}) T ] at h2
-  exact h2
-
--- lemma exists_cover (M : Matroid α) {k : ℕ∞} (hk : 1 ≤ k) :
---     ∃ T, M.IsCover k T ∧ T.encard = M.coverNumber k := by
---   simpa using csInf_mem <| (M.setOf_cover_nonempty hk).image encard
+  obtain ht | ⟨T, hT, hT' ⟩ := (X \ {e}).exists_cover (fun A ↦ (M ／ {e}).eRk A ≤ a)
+  · rw [ht]
+    exact OrderTop.le_top (X.coverNumber fun A ↦ M.eRk A ≤ a + 1)
+  have hcov : ((fun x ↦ x ∪ {e}) '' T).IsCover X fun A ↦ M.eRk A ≤ (a + 1) := by
+    have hrw : X = X \ {e} ∪ {e} := by grind
+    nth_rw 1 [hrw]
+    apply hT.contract hne (P' := (fun A ↦ M.eRk A ≤ a + 1)) (P := (fun A ↦ (M ／ {e}).eRk A ≤ a)) (X := {e})
+    intro F hF
+    --rw [@union_singleton]
+    rw [←eRelRk_eq_eRk_contract M {e} F] at hF
+    grw [ ←eRelRk_add_eRk_eq M {e} F, IsNonloop.eRk_eq hel]
+    simp only [ne_eq, ENat.one_ne_top, not_false_eq_true, add_le_add_iff_left_of_ne_top]
+    exact hF
+  grw [←hT', hcov.coverNumber_le]
+  simp only [union_singleton, ge_iff_le]
+  exact encard_image_le (fun a ↦ insert e a) T
 
 
-
--- lemma coverNumber_contract {a : ℕ∞} (hX : X ⊆ M.E) :
---     M.coverNumber (a + M.eRk X) ≤ (M ／ X).coverNumber a := by
---   --Mathieu, do you want to do this one?
---   sorry
-
--- def closZ (a : ℕ) (hx : X.Finite ) (hX : X ⊆ M.E)
---     (Y : (M ↾ F).closure '' { Y | Y ⊆ X ∧ M.eRk Y = a} )
---     : ∃ Z :  { Y | Y ⊆ X ∧ M.eRk Y = a}, Y.1 = Z.1 := by
---   have := (mem_image ((M ↾ F).closure) ({ Y | Y ⊆ X ∧ M.eRk Y = a}) Y.1  ).1 Y.2
---   obtain ⟨Y, hY ⟩ := (mem_image ((M ↾ F).closure) ({ Y | Y ⊆ X ∧ M.eRk Y = a}) Y.1  ).1 Y.2
---   sorry
-
--- def IsFlat.restriction_clo (hF : M.IsFlat F) (hY : Y ⊆ F) : M.closure Y = (M ↾ F).closure Y :=
---     by
---   sorry
-
-
-
---Dont need
--- def closZ (a : ℕ)
---     (Z : (M ↾ F).closure '' { Y | Y ⊆ X ∧ M.eRk Y = a} )
---     : ∃ Y :  { Y | Y ⊆ X ∧ M.eRk Y = a}, (M ↾ F).closure Y.1 = Z.1 := by
---   --have := (mem_image ((M ↾ F).closure) ({ Y | Y ⊆ X ∧ M.eRk Y = a}) Y.1  ).1 Y.2
---   obtain ⟨Y, hY, h ⟩ := (mem_image ((M ↾ F).closure) ({ Y | Y ⊆ X ∧ M.eRk Y = a}) Z.1  ).1 Z.2
---   use ⟨Y, hY⟩
-
--- def getI (a : ℕ) (hX : X ⊆ M.E)
---     (Y : { Y | Y ⊆ X ∧ M.eRk Y = a} )
---     : ∃ I : {Y | Y ⊆ X ∧ Y.encard = a}, I.1 ⊆ X ∧ (M.IsBasis I Y.1) ∧ I.1.encard = a := by
---   --have : Y ⊆ M.E := by sorry
---   obtain ⟨I, hIB, hc ⟩ := (M.eq_eRk_iff.1 Y.2.2)
---   have h' :  I ∈ {Y | Y ⊆ X ∧ Y.encard = ↑a} := by
---     refine ⟨LE.le.subset fun ⦃a⦄ a_2 ↦ (Y.2.1 ) (IsBasis.subset hIB  a_2) , hc ⟩
---   use ⟨ I, h' ⟩
---   refine ⟨h'.1, hIB , hc ⟩
-
--- def ranksubsets_Map (a : ℕ) (b : ℕ) (hx : X.Finite ) (hX : X ⊆ M.E) (hF : M.IsFlat F) (hXF : X ⊆ F)
---     : Function.Embedding
---     ((M ↾ F).closure '' { Y | Y ⊆ X ∧ M.eRk Y = a}) {Y | Y ⊆ X ∧ Y.encard = a} :=
--- --have := LE.le.subset fun ⦃a⦄ a_1 ↦ hX (hY.1 a_1)
--- { toFun := fun Z =>
---     ⟨ (Classical.choose (getI a hX (Classical.choose (closZ a Z ))) ).1 ,
---     (Classical.choose (getI a hX (Classical.choose (closZ a Z ))) ).2 ⟩
---   inj' := by
---     intro x y hxy
---     simp only [Subtype.mk.injEq] at hxy
---     have heq : x.1 = y.1 := by
---       rw[ ←(Classical.choose_spec (closZ a x )), ←(Classical.choose_spec (closZ a y )) ]
---       --simp only [mem_setOf_eq, coe_setOf ]
---       rw[←hF.restriction_clo ?_, ←hF.restriction_clo ?_,
---       ←((Classical.choose_spec (getI a hX (Classical.choose (closZ a x ))) ).2.1).closure_eq_closure,
---       ←((Classical.choose_spec (getI a hX (Classical.choose (closZ a y ))) ).2.1).closure_eq_closure,
---       hxy ]
---       --simp only [restrict_closure_eq']
---       --have := (Classical.choose_spec (getI a hX (Classical.choose (closZ a x ))) ).1
---       have := (Classical.choose (closZ a x )).2.1
---       --exact LE.le.subset fun ⦃b⦄ b_2 ↦ hXF (this b_2)
---       --grw[hXF] at this
---       --intro Y hY
-
---       --simp only [mem_setOf_eq, coe_setOf] at this
-
---       sorry
---       · sorry
---     exact SetCoe.ext heq
---     --rw[ ] at hxy
-
---     }
+lemma IsRankcoverNumber_contract_one' {a : ℕ∞} (hel : M.IsNonloop e) :
+    X.coverNumber (fun A ↦ M.eRk A ≤ (a + 1)) ≤ X.coverNumber (fun A ↦ (M ／ {e}).eRk A ≤ a)
+    := by
+  refine coverNumber_le_coverNumber (fun A ↦ (M ／ {e}).eRk A ≤ a) (fun A ↦ M.eRk A ≤ a + 1) X ?_
+  intro Y hY
+  simp only
+  intro h
+  rw [←eRelRk_eq_eRk_contract M {e} Y] at h
+  grw [eRk_subset_le M (subset_union_left (t := {e})), ←eRelRk_add_eRk_eq M {e} Y ]
+  rw[IsNonloop.eRk_eq hel ]
+  simp only [ne_eq, ENat.one_ne_top, not_false_eq_true, add_le_add_iff_left_of_ne_top, h]
 
 lemma set_to_binom_number {a b : ℕ} (X : Set α) (hX : X.encard = b) :
     {Y | Y ⊆ X ∧ Y.encard = a}.encard = b.choose a := by
@@ -641,60 +678,12 @@ lemma set_to_binom_number {a b : ℕ} (X : Set α) (hX : X.encard = b) :
     simpa
   rw [← ENat.coe_inj, ← hX, eq_comm, hXfin.encard_eq_coe_toFinset_card]
 
--- lemma base_isCover {a : ℕ} (hr : M.eRank ≤ a + 1) (ha : 1 ≤ a) (hXfin : X.Finite)
---     --(h : Maximal (fun Y ↦ Y ⊆ M.E ∧ (M ↾ Y).IsFiniteRankUniform (a + 1) Y.encard) X) :
---     (h : MaximalFor (fun x ↦ x ∈ {X | X ⊆ M.E ∧ (M ↾ X).IsFiniteRankUniform (a + 1) X.encard}) encard X) :
---     M.IsRankCover a (M.closure '' {K | K ⊆ X ∧ K.encard = a}) := by
---   refine ⟨?_, ?_⟩
---   · refine subset_antisymm (sUnion_subset fun K ↦ ?_) fun e he ↦ ?_
---     · simp only [mem_image, mem_setOf_eq, forall_exists_index, and_imp]
---       grind
---     obtain ⟨E, hEX, hEunif⟩ := h.prop.2.exists_eq_unifOn
---     obtain rfl : X = E := congr_arg Matroid.E hEunif
---     by_contra! hcon
---     simp only [sUnion_image, mem_setOf_eq, mem_iUnion, exists_prop, not_exists, not_and,
---       and_imp] at hcon
---     have hcon' (Z) (hZ : Z ⊆ X) (hZa : Z.encard ≤ a) : e ∉ M.closure Z := by
---       have haX : a ≤ X.encard := by
---         grw [← M.restrict_ground_eq (R := X), ← eRank_le_encard_ground, h.prop.2.eRank_eq]
---         simp
---       obtain ⟨W, hZW, hWZ, hW⟩ := exists_superset_subset_encard_eq hZ hZa haX
---       exact notMem_subset (M.closure_subset_closure hZW) (hcon W hWZ hW)
---     have heX : e ∉ X := by
---       by_contra hc
---       exact hcon' (singleton e) (singleton_subset_iff.mpr hc )
---         (by simp only [encard_singleton, ENat.one_le_coe, ha ]) (mem_closure_self M e he )
---     --have hwin := h.not_prop_of_ssuperset (t := insert e X) (by grind)
---     have hwin := h.not_prop_of_gt (j := insert e X)
---       (Finite.encard_lt_encard hXfin (ssubset_insert heX ))
---     simp only [mem_setOf_eq, not_and, insert_subset_iff.mpr ⟨he, h.prop.1 ⟩,forall_const ] at hwin
---     --rw [insert_subset_iff , and_iff_right he, and_iff_right h.prop.1] at hwin
---     apply hwin
---     suffices aux : (M ↾ insert e X) = unifOn (insert e X) (a + 1) by
---       rw [aux]
---       apply unifOn_isFiniteRank_uniform
---       grw [h.prop.2.le, ← subset_insert]
---     refine ext_indep rfl fun I (hI : I ⊆ insert e X) ↦ ?_
---     simp only [restrict_indep_iff, hI, and_true, unifOn_indep_iff, Nat.cast_add, Nat.cast_one]
---     refine ⟨fun hIi ↦ by grw [hIi.encard_le_eRank, hr], fun hcard ↦ ?_⟩
---     have hI₀ : M.Indep (I \ {e}) := by
---       have hrestr := (M.restrict_indep_iff (R := X) (I := I \ {e})).1
---       nth_grw 1 [hEunif, unifOn_indep_iff, diff_subset] at hrestr
---       grind
---     by_cases! heI : e ∉ I
---     · rwa [diff_singleton_eq_self heI] at hI₀
---     rw [← insert_diff_self_of_mem heI, hI₀.insert_indep_iff_of_notMem (by grind), mem_diff,
---       and_iff_right he]
---     refine hcon'  _ (by grind) ?_
---     grw [← ENat.add_one_le_add_one_iff, ← hcard, encard_diff_singleton_add_one heI]
---   simp only [mem_image, mem_setOf_eq, forall_exists_index, and_imp]
---   rintro F I hI hcard rfl
---   grw [eRk_closure_eq, eRk_le_encard, hcard]
-
+-- Do we want to do it with a set X?
 lemma base_isCover {a : ℕ} (hr : M.eRank ≤ a + 1) (ha : 1 ≤ a) (hXfin : X.Finite)
     --(h : Maximal (fun Y ↦ Y ⊆ M.E ∧ (M ↾ Y).IsFiniteRankUniform (a + 1) Y.encard) X) :
     (h : MaximalFor (fun x ↦ x ∈ {X | X ⊆ M.E ∧ (M ↾ X).IsFiniteRankUniform (a + 1) }) encard X) :
-    M.IsRankCover a (M.closure '' {K | K ⊆ X ∧ K.encard = a}) := by
+    M.IsRankCover (M.closure '' {K | K ⊆ X ∧ K.encard = a}) M.E a := by
+    --M.IsRankCover a (M.closure '' {K | K ⊆ X ∧ K.encard = a}) := by
   refine ⟨?_, ?_⟩
   · refine subset_antisymm (sUnion_subset fun K ↦ ?_) fun e he ↦ ?_
     · simp only [mem_image, mem_setOf_eq, forall_exists_index, and_imp]
@@ -747,7 +736,8 @@ lemma base_isCover {a : ℕ} (hr : M.eRank ≤ a + 1) (ha : 1 ≤ a) (hXfin : X.
 
 lemma baseCase {a b : ℕ} (ha : 1 ≤ a) (hM : NoUniformMinor M (a + 1) (b + 1))
     (hr : M.eRank = a + 1) :
-    M.coverNumber (fun M X ↦ M.eRk X ≤ a) ≤ Nat.choose b a := by
+    (M.E).coverNumber (fun A ↦ M.eRk A ≤ a ) ≤ Nat.choose b a := by
+    --M.coverNumber (fun M X ↦ M.eRk X ≤ a) ≤ Nat.choose b a := by
   have : M.RankFinite := M.eRank_ne_top_iff.mp (ENat.ne_top_iff_exists.2
       (Exists.intro ((fun x1 x2 ↦ x1 + x2) a 1) (hr.symm)))
   by_contra! hcon
@@ -794,13 +784,14 @@ lemma baseCase {a b : ℕ} (ha : 1 ≤ a) (hM : NoUniformMinor M (a + 1) (b + 1)
 
 lemma coverNumber_rank_Frombase {a b : ℕ} (ha : 1 ≤ a)
     (hM : NoUniformMinor M ( a + 1 ) (b + 1)) :
-    M.coverNumber (fun M X ↦ M.eRk X ≤ a) ≤
-    (Nat.choose b a) * M.coverNumber (fun M X ↦ M.eRk X ≤ (a + 1)) := by
+    (M.E).coverNumber (fun A ↦ M.eRk A ≤ a ) ≤
+    (Nat.choose b a) * (M.E).coverNumber (fun A ↦ M.eRk A ≤ (a + 1) ) := by
   sorry
 
 lemma coverNumber_Bound {M : Matroid α} [M.RankPos] {a b : ℕ} {n : ℕ∞} (ha : a ≠ 0) (hb : a ≤ b)
     (hM : NoUniformMinor M ( a + 1 ) (b + 1)) (hn : M.eRank = a + n) :
-    M.coverNumber (fun M X ↦ M.eRk X ≤ a) ≤ (Nat.choose b a)^(M.eRank - a) := by
+    (M.E).coverNumber (fun A ↦ M.eRk A ≤ a ) ≤ (Nat.choose b a)^(M.eRank - a) := by
+    --M.coverNumber (fun M X ↦ M.eRk X ≤ a) ≤ (Nat.choose b a)^(M.eRank - a) := by
   obtain htop | hfin := eq_or_ne M.eRank ⊤
   · grw [htop, ENat.top_sub_coe, ENat.epow_top, ← le_top]
     obtain rfl | hlt := hb.eq_or_lt
@@ -821,76 +812,19 @@ lemma coverNumber_Bound {M : Matroid α} [M.RankPos] {a b : ℕ} {n : ℕ∞} (h
   sorry
 termination_by M.eRank
 
-  -- suffices hn : ∀ n : ℕ, M.eRank = n + a + 1 →
-  --     M.coverNumber (fun M X ↦ M.eRk X ≤ a) ≤ (Nat.choose b a)^(n + 1 )
-  -- ·
-  --   sorry
-  -- intro n hn
-  -- induction n generalizing M with
-  -- | zero => sorry
-  -- | succ n IH => sorry
-
--- -- change `ha` to `a ≠ 0`.
--- lemma coverNumber_Bound_contract [M.RankFinite] {a b : ℕ} (ha : 1 ≤ a)
---     (hM : NoUniformMinor M ( a + 1 ) (b + 1)) (hC : C ⊂ M.E)  :
---     M.coverNumber (fun M X ↦ M.eRk X ≤ a) ≤
---     (Nat.choose b a)^(M.eRk C ) * (M／C).coverNumber (fun M X ↦ M.eRk X ≤ a) := by
---   suffices hn : ∀ n : ℕ, n = M.eRk C →  M.coverNumber (fun M X ↦ M.eRk X ≤ a) ≤
---       (Nat.choose b a)^n * (M／C).coverNumber (fun M X ↦ M.eRk X ≤ a)
---   · obtain ⟨ n, hh ⟩ := ENat.ne_top_iff_exists.1 ( eRk_ne_top (M := M) (X := C))
---     rw[←hh]
---     exact le_of_eq_of_le rfl (hn n hh)
---   intro n hn
---   induction n generalizing M C with
---   | zero =>
---     simp only [pow_zero, one_mul]
---     rw [coverNumber_contract_loop ((ground_nonempty_iff (M ＼ C)).mp (nonempty_of_ssubset hC ) )
---       (ENat.one_le_coe.mpr ha ) ((eRk_eq_zero_iff (subset_of_ssubset hC)).1 hn.symm )]
---   | succ n IH =>
---   grw[coverNumber_rank_Frombase ha hM ]
---   have hresP : (M ↾ C).RankPos :=
---     (eRank_ne_zero_iff (M ↾ C)).mp <| by simp [eRank_restrict, ne_eq, ← hn]
-
---   obtain ⟨e, heC ⟩ := exists_isNonloop (M ↾ C)
---   obtain ⟨heC1, heC2 ⟩ := restrict_isNonloop_iff.1 heC
---   have heN : (M／ {e}).Nonempty := by
---     rw[←(M／ {e}).ground_nonempty_iff, contract_ground]
---     exact (Set.nonempty_of_ssubset (by grind ) )
---   grw[ coverNumber_contract_one (heC1.mem_ground ) heC1 heN]
---   have hn1 : (M／ {e}).eRk (C \ {e}) = n := by
---     have hrelrk := IsNonloop.eRelRk_add_one_eq heC1 (C \ {e})
---     simp only [insert_diff_singleton, insert_eq_of_mem heC2, ←hn, Nat.cast_add, Nat.cast_one,
---       ne_eq, ENat.one_ne_top, not_false_eq_true,
---       add_left_inj_of_ne_top] at hrelrk
---     rwa [eRelRk.eq_1] at hrelrk
---   have hsub1 : (C \ {e}) ⊂ (M／ {e}).E := by
---     simp only [contract_ground]
---     refine Set.ssubset_iff_subset_ne.mpr ⟨diff_subset_diff_left (subset_of_ssubset hC), ?_ ⟩
---     by_contra hc
---     have h : C = M.E := by
---       rw [←insert_diff_self_of_mem heC2, ←insert_diff_self_of_mem heC1.mem_ground, hc]
---     have hCE : C ≠ M.E := by exact Std.ne_of_lt hC
---     rw [h] at hCE
---     exact false_of_ne hCE
---   grw[ IH (hM.minor (contract_isMinor M {e} )) hsub1 hn1.symm ]
---   simp only [contract_contract, union_diff_self, singleton_union, ge_iff_le, insert_eq_of_mem heC2,
---     ←mul_assoc ]
---   nth_rw 1 [ ←ENat.epow_one (x := ↑(b.choose a)), ←ENat.epow_natCast,
---     ←ENat.epow_add (x :=  ↑(b.choose a)) (y := 1) (z := n ), ←ENat.coe_one, ←ENat.coe_add,
---     ENat.epow_natCast, add_comm ]
-
-
--- change `ha` to `a ≠ 0`.
 lemma coverNumber_Bound_contract {M : Matroid α} {C : Set α} {a b : ℕ} (ha : a ≠ 0) (hb : a ≤ b)
     (hM : NoUniformMinor M (a + 1) (b + 1)) (hC : C ⊂ M.E)  :
-    M.coverNumber (fun M X ↦ M.eRk X ≤ a) ≤
-    (Nat.choose b a)^(M.eRk C) * (M ／ C).coverNumber (fun M X ↦ M.eRk X ≤ a) := by
+    (M.E).coverNumber (fun A ↦ M.eRk A ≤ a ) ≤
+    (Nat.choose b a)^(M.eRk C) * ((M ／ C).E).coverNumber (fun A ↦ (M ／ C).eRk A ≤ a ) := by
+    --M.coverNumber (fun M X ↦ M.eRk X ≤ a) ≤
+    --(Nat.choose b a)^(M.eRk C) * (M ／ C).coverNumber (fun M X ↦ M.eRk X ≤ a) := by
   obtain htop | hlt := eq_or_ne (M.eRk C) ⊤
   · grw [htop, ENat.epow_top, ENat.top_mul, ← le_top ]
     · have heN : (M／ C).Nonempty := by
         rw[←(M／ C).ground_nonempty_iff, contract_ground]
         exact (Set.nonempty_of_ssubset (by grind ) )
-      exact ENat.one_le_iff_ne_zero.mp (coverNumer_positive (fun M X ↦ M.eRk X ≤ a) )
+      exact ENat.one_le_iff_ne_zero.mp (coverNumber_positive
+        ((ground_nonempty_iff (M ／ C)).mpr heN) (fun A ↦ (M ／ C).eRk A ≤ a ) )
     obtain rfl | hlt := hb.eq_or_lt
     · simp [noUniformMinor_self_iff] at hM
       grw [ ←eRk_le_eRank M C, htop ] at hM
@@ -898,7 +832,13 @@ lemma coverNumber_Bound_contract {M : Matroid α} {C : Set α} {a b : ℕ} (ha :
     rw [← ENat.coe_one, ENat.coe_lt_coe]
     suffices b.choose a ≠ 0 ∧ b.choose a ≠ 1 by lia
     exact ⟨(Nat.choose_pos hlt.le).ne.symm, by simp [Nat.choose_eq_one_iff, hlt.ne.symm, ha] ⟩
-  have hresP : (M ↾ C).RankPos := sorry
+  obtain h0 | hn := eq_or_ne (M.eRk C) 0
+  · rw [h0]
+    simp only [ENat.epow_zero, contract_ground, one_mul]
+    --Need loop lemma
+    sorry
+  have hresP : (M ↾ C).RankPos := (eRank_ne_zero_iff (M ↾ C)).mp <|
+    by simp [eRank_restrict, ne_eq, hn]
     -- (eRank_ne_zero_iff (M ↾ C)).mp <| by simp [eRank_restrict, ne_eq, ← hn]
   obtain ⟨e, heC⟩ : ∃ e, (M ↾ C).IsNonloop e := exists_isNonloop (M ↾ C)
   rw [restrict_isNonloop_iff] at heC
@@ -927,59 +867,84 @@ lemma coverNumber_Bound_contract {M : Matroid α} {C : Set α} {a b : ℕ} (ha :
   have : 1 ≤ a := by exact Nat.one_le_iff_ne_zero.mpr ha
   have ih := coverNumber_Bound_contract (M := M ／ {e}) (C := C \ {e}) (a := a) (b := b) ha
     hb (hM.minor (contract_isMinor M {e} )) hsub1
-  grw [coverNumber_rank_Frombase (Nat.one_le_iff_ne_zero.mpr ha) hM, coverNumber_contract_one (heC.1.mem_ground ) heC.1 heN, ih ]
+  nth_rw 1 [contract_ground M {e} ] at ih
+  grw [coverNumber_rank_Frombase (Nat.one_le_iff_ne_zero.mpr ha) hM,
+    IsRankcoverNumber_contract_one heC.1 (mem_of_subset_of_mem (subset_of_ssubset hC ) (heC.2 ))
+    (nonempty_of_ssubset' hsub1 ), ih ]
   simp only [contract_contract, union_diff_self, singleton_union, ge_iff_le, insert_eq_of_mem heC.2,
     ←mul_assoc]
   nth_rw 1 [←eRelRk.eq_1, ←ENat.epow_one (x := ↑(b.choose a)),
     ←ENat.epow_add (x :=  ↑(b.choose a)) (y := 1) (z := (M.eRelRk {e} (C \ {e})) ),
-    ←add_comm (a := (M.eRelRk {e} (C \ {e}))) (b:= 1 ), (heC.1).eRelRk_add_one_eq, insert_diff_singleton, insert_eq_of_mem heC.2 ]
+    ←add_comm (a := (M.eRelRk {e} (C \ {e}))) (b:= 1 ),
+    (heC.1).eRelRk_add_one_eq, insert_diff_singleton, insert_eq_of_mem heC.2 ]
 
 termination_by M.eRk C
-
 
 end Rank
 
 section NonSpanning
 
-lemma NonSpanning_to_RankCover [M.RankFinite] (hM : 2 ≤ M.eRank) :
-    M.IsCover Matroid.Nonspanning T ↔ M.IsRankCover (M.eRank - 1) T := by
+def NonSpanningCover (M : Matroid α) (T : Set (Set α)) (X : Set α) :=
+    T.IsCover X (M ↾ X).Nonspanning
+
+lemma NonSpanningCover_iff : NonSpanningCover M T X ↔ T.IsCover X (M ↾ X).Nonspanning :=
+  Eq.to_iff rfl
+
+-- This should be shorter
+lemma NonSpanningCover_iff_restriction :
+    M.NonSpanningCover T X ↔ (M ↾ X).NonSpanningCover T (M ↾ X).E := by
+  refine ⟨?_, ?_ ⟩
+  · intro h
+    rw [NonSpanningCover_iff, restrict_ground_eq, restrict_idem]
+    exact NonSpanningCover_iff.mp h
+  intro h
+  rw [NonSpanningCover_iff, restrict_ground_eq, restrict_idem] at h
+  exact NonSpanningCover_iff.mpr h
+
+lemma NonSpanning_to_RankCover [M.RankFinite] (hM : 2 ≤ M.eRk X) :
+    NonSpanningCover M T X ↔ M.IsRankCover T X (M.eRk X - 1) := by
+    --M.IsCover Matroid.Nonspanning T ↔ M.IsRankCover (M.eRank - 1) T := by
   refine ⟨?_, ?_ ⟩
   · intro h
     refine ⟨ h.sUnion_eq, ?_ ⟩
     intro F hF
     by_contra hc
     simp only [not_le] at hc
-    have : M.eRank ≤ M.eRk F := by
-      have : M.eRank - 1 + 1 ≤  M.eRk F := by exact Order.add_one_le_of_lt hc
-      sorry
     sorry
   sorry
 
-lemma NonSpaning_le_two [M.Nonempty] (hle : M.eRank ≤ 1) :
-    ⊤ ≤ M.coverNumber (Matroid.Nonspanning) := by
-  obtain hT | ⟨T, hT1, hT2 ⟩  := M.exists_cover (Matroid.Nonspanning)
+lemma NonSpaning_le_two (hX : X.Nonempty) (hle : M.eRk X ≤ 1) :
+    ⊤ ≤ X.coverNumber (M ↾ X).Nonspanning := by
+  --rw [NonSpanningCover_iff]
+  obtain hT | ⟨T, hT1, hT2 ⟩  := X.exists_cover (M ↾ X).Nonspanning
+  --M.exists_cover (Matroid.Nonspanning)
   · rw[ hT ]
   by_contra hc
-  have : M.RankFinite := by
+  have : (M ↾ X).RankFinite := by
     refine eRank_lt_top_iff.mp ?_
+    simp only [eRank_restrict]
     grw[hle]
     exact ENat.one_lt_top
   have hu := hT1.sUnion_eq
-  have hl : ∀ T1 ∈ T, T1 ⊆ M.loops := by
+  have hl : ∀ T1 ∈ T, T1 ⊆ (M ↾ X).loops := by
     intro T1 hT'
-    have h1 : M.eRk T1 < M.eRank := Nonspanning.eRk_lt (hT1.pProp T1 hT' )
+    have h1 := Nonspanning.eRk_lt (hT1.pProp T1 hT' )
+    rw [←eRank_restrict] at hle
     grw [hle] at h1
+    --←restrict_eRk_eq M (hT1.subset hT'),
     simp only [ENat.lt_one_iff] at h1
-    exact (M.eRk_eq_zero_iff (X := T1) (hX := by grind)).1 h1
-  have hs : M.E ⊆ M.loops := by
-    rw [←hT1.sUnion_eq]
+    -- have hX : T1 ⊆ (M ↾ X).E := by exact IsCover.subset hT1 hT'
+    exact ((M ↾ X).eRk_eq_zero_iff (X := T1) (hT1.subset hT') ).1 h1
+  have hs : (M ↾ X).E ⊆ (M ↾ X).loops := by
+    nth_rw 1 [←hT1.sUnion_eq]
+    --rw [←hT1.sUnion_eq]
     exact sUnion_subset hl
-  obtain ⟨T', hT' ⟩ := hT1.nonempty
-  have h2 : M.E ⊆ M.closure T' := by
+  obtain ⟨T', hT' ⟩ := hT1.nonempty hX
+  have h2 : (M ↾ X).E ⊆ (M ↾ X).closure T' := by
     grw [hs]
-    exact loops_subset_closure M T'
+    exact loops_subset_closure (M ↾ X) T'
   exact Ne.elim (fun a ↦ ((hT1.pProp T' hT').not_spanning) ((spanning_iff_ground_subset_closure
-    (hT1.subset_ground hT') ).2 h2)) hT2
+    (hT1.subset hT') ).2 h2)) hT2
 
 
 lemma Non_spanning_singleton (he : e ∈ M.E) (hM : 2 ≤ M.eRank) : M.Nonspanning {e} := by
@@ -991,49 +956,132 @@ lemma Non_spanning_singleton (he : e ∈ M.E) (hM : 2 ≤ M.eRank) : M.Nonspanni
     grw [←hM] at h1
     simp only [ENat.not_ofNat_le_one] at h1
 
-lemma IsCover_singleton_NonSpanning (hM : 2 ≤ M.eRank) :
-    M.IsCover (Matroid.Nonspanning) (singleton '' M.E) := by
+lemma IsCover_singleton_NonSpanning (hM : 2 ≤ M.eRk X) :
+    NonSpanningCover M (singleton '' X) X := by
+    --M.IsCover (Matroid.Nonspanning) (singleton '' M.E) := by
   exact IsCover_singleton_Prop (fun e he ↦ Non_spanning_singleton he hM)
 
-lemma IsCover_singleton_le_NonSpanning (hM : 2 ≤ M.eRank) :
-    M.coverNumber (Matroid.Nonspanning) ≤ M.E.encard := by
+lemma IsCover_singleton_le_NonSpanning (hM : 2 ≤ M.eRk X) :
+    X.coverNumber ((M ↾ X).Nonspanning) ≤ X.encard := by
   exact IsCover_singleton_le (fun e he ↦ Non_spanning_singleton he hM)
 
-lemma NonSpaning_cover_exists (hM : 2 ≤ M.eRank) : M.hasCover_with Matroid.Nonspanning := by
-  refine ⟨(singleton '' M.E), IsCover_singleton_NonSpanning hM ⟩
+lemma NonSpaning_cover_exists (hM : 2 ≤ M.eRk X) : X.hasCover_with ((M ↾ X).Nonspanning) := by
+  refine ⟨(singleton '' X), IsCover_singleton_NonSpanning hM ⟩
 
-lemma IsNonSpaningCover_contract (h : (M ／ X).IsCover (Matroid.Nonspanning) T)
-    (hX : X ⊆ M.E) (hXN : (M ／ X).Nonempty) :
-    M.IsCover (Matroid.Nonspanning) ((· ∪ X) '' T) := by
-  apply h.contract hX hXN
-  intro Y hC
-  refine ⟨ ?_, union_subset (by have := hC.subset_ground; grind ) hX  ⟩
-  · by_contra hc
-    have hcc : (M ／ X).Spanning Y := by
-      have h1 := hc.contract X
-      simp only [union_diff_right] at h1
-      exact h1.superset (diff_subset (s := Y) (t := X)) (hC.subset_ground)
-    rw [←not_spanning_iff hcc.subset_ground ] at hC
-    exact (iff_false_intro hC).mp hcc
+lemma IsNonSpaningCover_contract (h : NonSpanningCover (M ／ C) T (M.E \ C))
+    --(h : (M ／ X).IsCover (Matroid.Nonspanning) T)
+    (hX : C ⊆ M.E) (hXN : (M ／ C).Nonempty) :
+    NonSpanningCover M ((· ∪ C) '' T) M.E := by
+  rw [NonSpanningCover_iff] at h
+  rw [NonSpanningCover_iff]
+  have : (M.E \ C ∪ C) = M.E := by grind
+  nth_rw 1 [← this]
+  rw [←Matroid.ground_nonempty_iff, contract_ground] at hXN
+  apply h.contract (X := C) hXN
+  intro F hF
+  have h3 :  (M ／ C ↾ M.E \ C) = M ／ C := by
+    simp only [restrict_eq_self_iff, contract_ground]
+  rw [h3] at hF
+  simp only [restrict_ground_eq_self]
+  by_contra hc
+  have hcc : (M ／ C).Spanning F := by
+    have hr : F ∪ C ⊆ M.E := by
+      refine union_subset ?_ hX
+      have := hF.subset_ground
+      grind
+    rw [not_nonspanning_iff hr] at hc
+    refine (contract_spanning_iff hX).mpr ⟨hc, by grind ⟩
+  rw [←not_spanning_iff (hF.subset_ground)] at hF
+  exact Ne.elim (fun a ↦ hF hcc) h3
 
-lemma NonSpanningNumber_contract (hX : X ⊆ M.E) (hne : (M ／ X).Nonempty) :
-    M.coverNumber Matroid.Nonspanning ≤ (M ／ X).coverNumber Matroid.Nonspanning := by
-  obtain hT | ⟨T, hT, hTe ⟩ := (M ／ X).exists_cover (Matroid.Nonspanning)
+lemma IsNonSpaningCover_contract_subset (h : NonSpanningCover (M ／ C) T (Y \ C) )
+    (hX : C ⊆ Y) (hY : (Y \ C).Nonempty) :
+    NonSpanningCover M ((· ∪ C) '' T) Y := by
+  have h1 : NonSpanningCover ( (M ↾ Y) ／ C) T (((M ↾ Y)).E \ C) := by
+    simp only [restrict_ground_eq]
+    refine ⟨h.sUnion_eq , ?_ ⟩
+    intro F  hF
+    rw [restrict_contract_eq_contract_restrict M hX, restrict_idem]
+    exact h.pProp F hF
+  rw [NonSpanningCover_iff_restriction ]
+  exact IsNonSpaningCover_contract h1 (IsLoopEquiv.subset_ground rfl hX )
+    ((ground_nonempty_iff ((M ↾ Y) ／ C)).mp hY )
+
+-- lemma IsNonSpaningCover_contract_subset' (h : NonSpanningCover (M ／ C) T Y )
+--     (hY : Y.Nonempty) :
+--     NonSpanningCover M ((· ∪ C) '' T) (Y ∪ C) := by
+--   rw [NonSpanningCover_iff] at h
+--   rw [NonSpanningCover_iff]
+--   apply h.contract (X := C) hY
+--   intro F hF
+--   by_contra hc
+--   have hcc : (M ／ C ↾ Y).Spanning F := by
+--     have hr : F ∪ C ⊆ (M ↾ (Y ∪ C)).E := by
+--       simp only [restrict_ground_eq, union_subset_iff, subset_union_right, and_true]
+--       exact subset_union_of_subset_left hF.subset_ground C
+--     rw [not_nonspanning_iff hr] at hc
+--     -- have hhY : Y ⊆ (M ／ C).E := by
+--     --   simp only [contract_ground]
+--     --   sorry
+--     -- apply (restrict_spanning_iff (hF.subset_ground) ).2
+--     refine ⟨?_, ?_ ⟩
+--     sorry
+--     --simp only [restrict_closure_eq, contract_closure_eq, contract_ground, restrict_ground_eq]
+
+--     --simp only [union_diff_right] at h1
+
+--     sorry
+--   rw [←not_nonspanning_iff (hF.subset_ground)] at hcc
+--   exact (iff_false_intro hcc).mp hF
+
+  --rw [←Matroid.ground_nonempty_iff, contract_ground] at hY
+
+lemma NonSpanningNumber_contract (hX : C ⊆ M.E) (hXN : (M ／ C).Nonempty) :
+    M.E.coverNumber M.Nonspanning ≤ (M.E \ C).coverNumber (M ／ C).Nonspanning := by
+  obtain hT | ⟨T, hT, hTe ⟩ := (M.E \ C).exists_cover (M ／ C).Nonspanning
   · rw [hT]
-    exact OrderTop.le_top (M.coverNumber Nonspanning)
+    exact OrderTop.le_top (M.E.coverNumber M.Nonspanning)
   rw [← hTe]
+  rw [←(restrict_ground_eq_self (M ／ C)), contract_ground M C,
+    ←NonSpanningCover_iff (T := T ) (X := M.E \ C) (M := M ／ C)] at hT
+  have hrw2 := ((IsNonSpaningCover_contract hT hX hXN).coverNumber_le)
+  simp only [restrict_ground_eq_self] at hrw2
   exact
-    Std.IsPreorder.le_trans (M.coverNumber Nonspanning) ((fun x ↦ x ∪ X) '' T).encard T.encard
-      ((IsNonSpaningCover_contract hT hX hne).coverNumber_le)
-      (encard_image_le (fun x ↦ x ∪ X) T )
+    Std.IsPreorder.le_trans (M.E.coverNumber M.Nonspanning) ((fun x ↦ x ∪ C) '' T).encard T.encard
+      hrw2 (encard_image_le (fun x ↦ x ∪ C) T )
+
+lemma NonSpanningNumber_contract_subset (hX : C ⊆ Y) (hYne : (Y \ C).Nonempty) :
+    Y.coverNumber (M ↾ Y).Nonspanning ≤ (Y \ C).coverNumber ((M ／ C) ↾ (Y \ C)).Nonspanning := by
+  obtain hT | ⟨T, hT, hTe ⟩ := (Y \ C).exists_cover ((M ／ C) ↾ (Y \ C)).Nonspanning
+  · rw [hT]
+    exact OrderTop.le_top (Y.coverNumber (M ↾ Y).Nonspanning)
+  rw [← hTe]
+  rw [←NonSpanningCover_iff (T := T ) (X := Y \ C) (M := M ／ C)] at hT
+  exact
+    Std.IsPreorder.le_trans (Y.coverNumber (M ↾ Y).Nonspanning) ((fun x ↦ x ∪ C) '' T).encard T.encard
+      ((IsNonSpaningCover_contract_subset hT hX hYne).coverNumber_le)
+      (encard_image_le (fun x ↦ x ∪ C) T )
+
+-- lemma NonSpanningNumber_contract_subset' (hYne : (Y \ C).Nonempty) :
+--     Y.coverNumber (M ↾ Y).Nonspanning ≤ Y.coverNumber ((M ／ C) ↾ Y).Nonspanning := by
+--   obtain hT | ⟨T, hT, hTe ⟩ := Y.exists_cover ((M ／ C) ↾ Y).Nonspanning
+--   · rw [hT]
+--     exact OrderTop.le_top (Y.coverNumber (M ↾ Y).Nonspanning)
+--   rw [← hTe]
+--   rw [←NonSpanningCover_iff (T := T ) (X := Y ) (M := M ／ C)] at hT
+--   have := (IsNonSpaningCover_contract_subset' hT hYne)
+--   exact
+--     Std.IsPreorder.le_trans (Y.coverNumber (M ↾ Y).Nonspanning) ((fun x ↦ x ∪ C) '' T).encard T.encard
+--       ((IsNonSpaningCover_contract_subset hT hX hYne).coverNumber_le)
+--       (encard_image_le (fun x ↦ x ∪ C) T )
 
 lemma NonSpanningNumber_set_closure (hY : Y ⊆ M.closure X) (hX : X ⊆ M.E) :
-    (M ↾ X).coverNumber Nonspanning  ≤ (M ↾ (X ∪ Y)).coverNumber Nonspanning := by
-  obtain hT | ⟨T, hT, hTe ⟩ := (M ↾ (X ∪ Y)).exists_cover (Matroid.Nonspanning)
+    X.coverNumber (M ↾ X).Nonspanning  ≤ (X ∪ Y).coverNumber (M ↾ (X ∪ Y)).Nonspanning := by
+  obtain hT | ⟨T, hT, hTe ⟩ := (X ∪ Y).exists_cover (M ↾ (X ∪ Y)).Nonspanning
   · rw [hT]
-    exact OrderTop.le_top ((M ↾ X).coverNumber Nonspanning)
+    exact OrderTop.le_top (X.coverNumber (M ↾ X).Nonspanning)
   rw[←hTe]
-  have hcov : (M ↾ X).IsCover (Matroid.Nonspanning) ((fun x ↦ x ∩ X) '' T) := by
+  have hcov : NonSpanningCover M ((fun x ↦ x ∩ X) '' T) X := by
     refine ⟨?_, ?_ ⟩
     · refine subset_antisymm (sUnion_subset fun K ↦ ?_) fun e he ↦ ?_
       · intro hK
@@ -1041,8 +1089,6 @@ lemma NonSpanningNumber_set_closure (hY : Y ⊆ M.closure X) (hX : X ⊆ M.E) :
         rw [← hK']
         grind
       have h1 := hT.sUnion_eq
-      simp only [restrict_ground_eq] at h1
-      simp only [restrict_ground_eq] at he
       have : e ∈  ⋃₀ T := by grind
       obtain ⟨ T', hT', heT' ⟩ := this
       have : e ∈ T' ∩ X := by grind
@@ -1058,57 +1104,1091 @@ lemma NonSpanningNumber_set_closure (hY : Y ⊆ M.closure X) (hX : X ⊆ M.E) :
       (closure_subset_closure M (inter_subset_left )) ((LE.le.subset fun ⦃a⦄ a_1 ↦
       (closure_subset_closure_of_subset_closure hc ) (hY a_1) ) a_1))
     rw [←restrict_spanning_iff (hR := by grind), ←not_nonspanning_iff (by grind)  ] at hcc
+    have := (hT.pProp F' hF')
     exact Ne.elim (fun a ↦ hcc (hT.pProp F' hF')) hTe
-    exact LE.le.subset (hT.subset_ground hF')
+    exact LE.le.subset (hT.subset hF')
   grw [hcov.coverNumber_le ]
   exact encard_image_le (fun x ↦ x ∩ X) T
 
+end NonSpanning
 
 
--- lemma NonSpaningNumber_delete_loop (hne : (M ＼ D).Nonempty) (hk : 1 ≤ k) (hD : D ⊆ M.loops ) :
---     M.coverNumber (fun M X ↦ M.eRk X ≤ k) = (M ＼ D).coverNumber (fun M X ↦ M.eRk X ≤ k) := by
+
+
+
+
+
+-- variable {α : Type*} {M N M' : Matroid α} {I F X Y F' F₀ F₁ F₂ P L H H₁ H₂ H' B C D K : Set α}
+--   {e f : α} {l r : ℕ} {a k : ℕ∞} {T : Set (Set α)} {ι : Type*} {i j : ι}
+--   {P P' : Matroid α → Set α → Prop}
+
+-- section General
+
+
+
+
+-- @[mk_iff]
+-- structure IsCover (M : Matroid α) (P : Matroid α → Set α → Prop) (T : Set (Set α)) : Prop where
+--   sUnion_eq : ⋃₀ T = M.E
+--   pProp : ∀ F ∈ T, P M F
+
+-- lemma IsCover.subset_ground (h : M.IsCover P T) (hX : X ∈ T) : X ⊆ M.E := by
+--   grw [← h.sUnion_eq, ← subset_sUnion_of_mem hX]
+
+-- -- monotone
+-- -- PCover iff ∀ e, ∃ X ∈ T, e ∈ X
+
+-- --Monotone under restriction
+-- def IsMRProp (P : Matroid α → Set α → Prop) : Prop :=
+--     ∀ M : Matroid α, ∀ F : Set α, ∀ Y : Set α, Y ⊆ F → P (M ↾ F) Y → P M Y
+
+-- --Monotone under subset
+-- def IsMSProp (P : Matroid α → Set α → Prop) : Prop :=
+--     ∀ M : Matroid α, ∀ F : Set α, ∀ Y : Set α, Y ⊆ F → P M F → P M Y
+
+-- -- --Minor union different prop. I think I want something different
+-- -- def IsMUProp (P : Matroid α → Set α → Prop) (P' : Matroid α → Set α → Prop) : Prop :=
+-- --     ∀ M : Matroid α, ∀ X : Set α, ∀ Y : Set α, P (M ／ X) Y → P' M (Y ∪ X)
+
+-- --Minor monotono
+-- -- def IsMMProp (P : Matroid α → Set α → Prop) (P' : Matroid α → Set α → Prop) : Prop :=
+-- --     --∀ M : Matroid α, ∀ X : Set α, ∀ Y : Set α, P (M ／ X) Y → P' M (Y ∪ X)
+-- --     ∀ N, N ≤m M → ∀ Y, Y ⊆ N.E → P N Y → P' M Y
+
+-- -- M has a cover with respect to prop P
+-- def hasCover_with (M : Matroid α) (P : Matroid α → Set α → Prop) : Prop :=
+--     ∃ T, M.IsCover P T
+
+-- lemma Cover_Nonempt_iff :
+--     M.hasCover_with P ↔ {T | M.IsCover P T}.Nonempty := by
+--   refine ⟨ fun a ↦ Nonempty.mono (fun ⦃a⦄ a_1 ↦ a_1) a , fun a ↦ ((fun a_1 ↦ a) ∘ fun a ↦ α) α ⟩
+
+-- lemma IsCover.nonempty [M.Nonempty] (h : M.IsCover P T) : T.Nonempty := by
+--   rw [nonempty_iff_empty_ne]
+--   rintro rfl
+--   simp [isCover_iff, eq_comm, M.ground_nonempty.ne_empty] at h
+
+-- lemma IsCover.one_le [M.Nonempty] (h : M.IsCover P T) : 1 ≤ T.encard := by
+--   simp only [one_le_encard_iff_nonempty]
+--   exact nonempty h
+
+-- noncomputable def coverNumber (M : Matroid α) (P : Matroid α → Set α → Prop) : ℕ∞ :=
+--     sInf (encard '' {T | M.IsCover P T})
+
+-- lemma coverNumber_eq_iInf (M : Matroid α) (P : Matroid α → Set α → Prop) :
+--     M.coverNumber P = ⨅ T ∈ {T | M.IsCover P T}, T.encard := by
+--   exact sInf_image
+
+-- lemma IsCover.coverNumber_le {T} (h : M.IsCover P T) : M.coverNumber P ≤ T.encard := by
+--   grw [coverNumber_eq_iInf]
+--   exact biInf_le encard h
+
+-- lemma exists_mincover_NE {M : Matroid α} {P : Matroid α → Set α → Prop}
+--     (hn : {T | M.IsCover P T}.Nonempty) :
+--     ∃ T, M.IsCover P T ∧ T.encard = M.coverNumber P := by
+--   simpa using csInf_mem <| hn.image encard
+
+-- lemma exists_min_cover {M : Matroid α} {P : Matroid α → Set α → Prop} (hP : M.hasCover_with P) :
+--     ∃ T, M.IsCover P T ∧ T.encard = M.coverNumber P := by
+--   simpa using csInf_mem <| (Cover_Nonempt_iff.1 hP ).image encard
+
+-- lemma exists_cover (M : Matroid α) (P : Matroid α → Set α → Prop) :
+--     M.coverNumber P = ⊤ ∨ ∃ T, M.IsCover P T ∧ T.encard = M.coverNumber P := by
+--   obtain h0 | h := {T | M.IsCover P T}.eq_empty_or_nonempty
+--   · simp [coverNumber_eq_iInf, h0]
+--   right
+--   simpa using csInf_mem <| h.image encard
+
+-- lemma coverNumer_positive [M.Nonempty] (P : Matroid α → Set α → Prop) :
+--     1 ≤ M.coverNumber P := by
+--   by_contra hc
+--   have h1 := ENat.lt_one_iff_eq_zero.mp (Std.not_le.mp hc)
+--   obtain ht | ⟨T, hT, hTe ⟩ := exists_cover M P
+--   · rw [h1] at ht
+--     simp only [ENat.zero_ne_top] at ht
+--   have := hT.nonempty
+--   grind
+
+-- lemma IsCover.cover_fun {M : Matroid α} {P' : Matroid α → Set α → Prop} (hP' : IsMRProp P')
+--     (hcover : M.IsCover P T)
+--     (f : Set α → Set (Set α) )
+--     (hfun : ∀ X ∈ T, (M ↾ X).IsCover P' (f X)) :
+--     M.IsCover P' ( ⋃ X ∈ T, f X ):= by
+--   refine ⟨ ?_, ?_ ⟩
+--   · rw[←hcover.sUnion_eq]
+--     refine ext ?_
+--     intro e
+--     refine ⟨ ?_, ?_ ⟩
+--     · intro he
+--       simp only [ mem_sUnion, mem_iUnion] at he
+--       obtain ⟨T', ⟨ X, ⟨hX, hT'X ⟩ ⟩, hee ⟩ := he
+--       simp only [mem_sUnion]
+--       refine ⟨ X ,⟨ hX , mem_of_subset_of_mem ((hfun X hX).subset_ground hT'X ) hee  ⟩ ⟩
+--     intro he
+--     simp only [mem_sUnion] at he
+--     obtain ⟨X, hXT, heX⟩ := he
+--     simp only [mem_sUnion, mem_iUnion]
+--     have h1 : e ∈ (M ↾ ↑X).E := by exact mem_of_subset_of_mem (fun ⦃a⦄ a_1 ↦ a_1) heX
+--     rw[←(hfun X hXT ).sUnion_eq] at h1
+--     simp only [mem_sUnion] at h1
+--     obtain ⟨X', hX', heX' ⟩ := h1
+--     refine ⟨ X', ⟨⟨X, ⟨hXT, hX'⟩ ⟩, heX'⟩ ⟩
+--   intro F hF
+--   simp only [ mem_iUnion] at hF
+--   obtain ⟨X, hXT, hF⟩ := hF
+--   exact hP' M X F (LE.le.subset ((hfun X hXT).subset_ground hF ) ) ((hfun X hXT).pProp F hF)
+
+
+-- lemma IsCover.cover_typset {P' : Matroid α → Set α → Prop} (hP' : IsMRProp P' )
+--     (hcover : M.IsCover P T )
+--     (f : T → Set (Set α) )
+--     (hfun : ∀ X : T, (M ↾ X.1).IsCover P' (f X)) :
+--     M.IsCover P' (⋃ X : T, f X ):= by
+--   refine ⟨ ?_, ?_ ⟩
+--   · rw[←hcover.sUnion_eq]
+--     refine ext ?_
+--     intro e
+--     refine ⟨ ?_, ?_ ⟩
+--     · intro he
+--       simp only [iUnion_coe_set, mem_sUnion, mem_iUnion] at he
+--       obtain ⟨T', ⟨ X, ⟨hX, hT'X ⟩ ⟩, hee ⟩ := he
+--       simp only [mem_sUnion]
+--       refine ⟨X, ⟨hX, (mem_of_subset_of_mem (((hfun ⟨X, hX⟩ ).subset_ground hT'X)) hee ) ⟩⟩
+--     intro he
+--     simp only [mem_sUnion] at he
+--     obtain ⟨X, hXT, heX⟩ := he
+--     simp only [iUnion_coe_set, mem_sUnion, mem_iUnion]
+--     have h1 : e ∈ (M ↾ ↑X).E := by exact mem_of_subset_of_mem (fun ⦃a⦄ a_1 ↦ a_1) heX
+--     rw[←(hfun ⟨X, hXT⟩ ).sUnion_eq] at h1
+--     simp only [mem_sUnion] at h1
+--     obtain ⟨X', hX', heX' ⟩ := h1
+--     refine ⟨ X', ⟨⟨X, ⟨hXT, hX'⟩ ⟩, heX'⟩ ⟩
+--   intro F hF
+--   simp only [iUnion_coe_set, mem_iUnion] at hF
+--   obtain ⟨X, hXT, hF⟩ := hF
+--   exact hP' M X F (LE.le.subset ((hfun ⟨X, hXT⟩).subset_ground hF ) ) ((hfun ⟨X, hXT⟩).pProp F hF)
+
+-- lemma coverNumber_cover_of_covers {P' : Matroid α → Set α → Prop} (hcover : M.IsCover P T)
+--     (hP' : IsMRProp P') :
+--     M.coverNumber P' ≤ ∑' X : T, (M ↾ X.1).coverNumber P' := by
+--   obtain (h0 | h1) := exists_or_forall_not (fun X : T ↦ (M ↾ X).coverNumber P' = ⊤)
+--   · simp [ENat.tsum_eq_top_of_eq_top h0]
+--   have hf : ∀ X : T, ∃ XT, (M ↾ X.1).IsCover P' XT ∧
+--     XT.encard = (M ↾ X.1).coverNumber P' := by
+--     intro X
+--     obtain (h | ⟨XT, hXres, hencard⟩) := (M ↾ X).exists_cover P'
+--     · simp [h1 _ h]
+--     exact ⟨XT, hXres, hencard⟩
+--   choose f hfunco hfunca using hf
+--   have hcover := IsCover.cover_typset hP' hcover f hfunco
+--   grw [hcover.coverNumber_le, ENat.encard_iUnion_le_tsum_encard, tsum_congr hfunca]
+
+-- lemma coverNumber_cover_of_covers_bound {P' : Matroid α → Set α → Prop} {k : ℕ∞}
+--     (hcover : M.IsCover P T) (hP' : IsMRProp P')
+--     (hflat : ∀ F, P M F → (M ↾ F).coverNumber P' ≤ k) :
+--     M.coverNumber P' ≤ (T.encard) * k := by
+--   grw [coverNumber_cover_of_covers hcover, ENat.tsum_le_tsum (g := fun _ ↦ k),
+--     ENat.tsum_subtype_const, mul_comm]
+--   intro F
+--   simp [hflat _ <| hcover.pProp F F.2 ]
+--   exact hP'
+
+
+-- --P is minor preserved wrt f if
+-- def MRProp (α) (P : Matroid α → Set α → Prop) (f : Set α → Matroid α → Set α → Prop ) : Prop :=
+--     ∀ M : Matroid α, ∀ Y X : Set α,
+--     ∃ (Q : Matroid α → Set α → Prop) , (P (M ／ Y) X → Q M X ∧ Q M X = f Y M X)
+
+-- --Help
+-- lemma RankIsMRProp (α) {k : ℕ∞} : MRProp (α)
+--     (fun M X ↦ M.eRk X ≤ k) (fun Y M X ↦ M.eRk (X ∪ Y) ≤ M.eRk Y + k ) := by
+--   intro M Y X
+--   use (fun N Z ↦ M.eRk (X ∪ Y) ≤ M.eRk Y + k )
+--   simp only [and_true]
 
 --   sorry
-  -- obtain ⟨T, hT, hTen ⟩ := exists_min_cover (RankPropCover_exists (M := M) hk )
-  -- have h1 := (hT.delete D ).coverNumber_le
-  -- grw[encard_image_le (fun s ↦ s \ D) T, hTen ] at h1
-  -- obtain ⟨T', hT', hT'en ⟩ := exists_min_cover (RankPropCover_exists (M := (M ＼ D)) hk )
-  -- have hcov : M.IsCover (fun M X ↦ M.eRk X ≤ k) (M.closure '' T' ) := by
-  --   refine ⟨ ?_, ?_ ⟩
-  --   · refine subset_antisymm (sUnion_subset fun K ↦ ?_) fun e he ↦ ?_
-  --     · simp only [mem_image, forall_exists_index, and_imp]
-  --       grind
-  --     by_cases heD : e ∈ D
-  --     · obtain ⟨ X, hX ⟩ := hT'.nonempty
-  --       have := (IsLoop.mem_closure (hD heD) X )
-  --       grind
-  --     have h2 : e ∈ M.E \ D := mem_diff_of_mem he heD
-  --     rw[←delete_ground,  ←hT'.sUnion_eq  ] at h2
-  --     obtain ⟨ X, hX, heX ⟩ := h2
-  --     have := (mem_closure_of_mem' M heX he )
-  --     grind
-  --   intro F hF
-  --   obtain ⟨F' ,hF', hF2 ⟩ := hF
-  --   rw[←hF2, eRk_closure_eq M F']
-  --   have ha := hT'.pProp F' hF'
-  --   simp only [delete_eRk_eq'] at ha
-  --   have ha1 : F' \ D = F' := by
-  --     have := hT'.subset_ground hF'
-  --     grind
-  --   rwa [ha1] at ha
-  -- have h2 := hcov.coverNumber_le
-  -- grw [encard_image_le M.closure T', hT'en] at h2
-  -- grind
 
--- lemma NonSpaningNumber_contract_loop (hne : (M ＼ D).Nonempty) (hk : 1 ≤ k) (hD : D ⊆ M.loops ) :
---     M.coverNumber (fun M X ↦ M.eRk X ≤ k) = (M ／ D).coverNumber (fun M X ↦ M.eRk X ≤ k) := by
---   rw[contract_eq_delete_of_subset_loops hD]
---   exact coverNumber_delete_loop hne hk hD
+-- -- --Minor preserved under f
+-- -- --(f : Set α → Matroid α → (Set α → Prop))
+-- -- def IsMUProp (P : Matroid α → Set α → Prop) (X : Set α ) (P' : Matroid α → Set α → Prop): Prop :=
+-- --     --∀ X : Set α,
+-- --     --∃ P' : Matroid α → Set α → Prop,
+-- --     ∀ M : Matroid α,
+-- --     ∀ Y : Set α, P (M ／ X) Y → P' M Y
+
+-- --P ' = k + M.eRk X for rank
+-- lemma IsCover.contract (h : (M ／ X).IsCover P T)
+--     (hX : X ⊆ M.E) (hXN : (M ／ X).Nonempty)
+--     (hPP' : ∀ Y : Set α, P (M ／ X) Y → P' M ( Y ∪ X) ) :
+--     M.IsCover P' ((· ∪ X) '' T) := by
+--   suffices hi : ∀ F ∈ T, P (M ／ X) F by
+--     simp only [isCover_iff, sUnion_image, mem_image, forall_exists_index, and_imp,
+--       forall_apply_eq_imp_iff₂, ← biUnion_distrib_union _ h.nonempty, ← sUnion_eq_biUnion,
+--       h.sUnion_eq, contract_ground, diff_union_self, union_eq_left, hX, true_and ]
+--     exact fun F hFT ↦ (((fun a ↦ (hPP' F (hi F hFT))) ∘ T) X )
+--   exact fun F hFT ↦ h.pProp F hFT
 
 
+-- --Close under closure
+-- def IsCCProp (α) (P : Matroid α → Set α → Prop) : Prop :=
+--     ∀ M : Matroid α, ∀ F : Set α, P M F → P M (M.closure F)
+
+-- lemma IsCover.isCover_closure (h : M.IsCover P T) (hP : IsCCProp α P) :
+--     M.IsCover P (M.closure '' T) := by
+--   simp only [isCover_iff, sUnion_image, subset_antisymm_iff (b := M.E), iUnion_subset_iff,
+--     M.closure_subset_ground, implies_true, true_and, mem_image, forall_exists_index, and_imp,
+--     forall_apply_eq_imp_iff₂]
+--   grw [h.sUnion_eq.symm.subset, sUnion_eq_biUnion]
+--   refine  ⟨biUnion_mono rfl.subset fun X hX ↦ M.subset_closure X (h.subset_ground hX),
+--   fun F hF ↦ (hP M F (h.pProp F hF)) ⟩
+
+-- --Singleton section
+-- -- noncomputable def SetsingletonEmbedding ( A : Set α ) : Function.Embedding
+-- --     {X : Set α // ∃ e ∈ A, {e} = X} {e // e ∈ A} :=
+-- -- { toFun := fun x => ⟨Classical.choose x.2, (Classical.choose_spec x.2).1 ⟩
+-- --   inj' := by
+-- --     intro x y hxy
+-- --     simp only [Subtype.mk.injEq] at hxy
+-- --     have heq : x.1 = y.1 := by
+-- --       rw [←(Classical.choose_spec x.2).2, ←(Classical.choose_spec y.2).2]
+-- --       exact singleton_eq_singleton_iff.mpr hxy
+-- --     exact Subtype.ext heq
+-- --     }
+
+-- lemma IsCover_singleton_Prop (hP : ∀ e ∈ M.E, P M (singleton e)) :
+--     M.IsCover P (singleton '' M.E) := by
+--   refine ⟨ ?_, ?_ ⟩
+--   · refine Eq.symm (ext ?_)
+--     intro x
+--     refine ⟨ ?_, ?_ ⟩
+--     · intro hx
+--       refine mem_sUnion.mpr ⟨{x} , ⟨ ?_ , mem_singleton x ⟩ ⟩
+--       use x
+--     intro hc
+--     simp only [sUnion_image, biUnion_of_singleton] at hc
+--     exact mem_of_subset_of_mem (fun ⦃a⦄ a_1 ↦ a_1) hc
+--   intro F hF
+--   obtain ⟨e, heE, heF ⟩ := hF
+--   rw[←heF]
+--   exact hP e heE
 
 
-end NonSpanning
+-- lemma IsCover_singleton_le (hP : ∀ e ∈ M.E, P M (singleton e)) :
+--     M.coverNumber P ≤ M.E.encard := by
+--   grw [(IsCover_singleton_Prop hP).coverNumber_le ]
+--   set Sing : Set (Set α ) := { singleton e | e ∈ M.E} with hs
+--   exact encard_image_le singleton M.E
+
+
+-- lemma IsCover.mono_prop (h : M.IsCover P T) (hPP' : ∀ X ∈ T, P M X → P' M X) : M.IsCover P' T :=
+--   (M.isCover_iff P' T).2 ⟨h.sUnion_eq, fun F hF ↦ hPP' F hF (h.pProp F hF)⟩
+
+-- lemma IsCover_emptyset_iff (P : Matroid α → Set α → Prop) : M.IsCover P ∅ ↔ ¬M.Nonempty := by
+--   refine ⟨?_, ?_ ⟩
+--   · intro h
+--     rw [ ←Matroid.ground_nonempty_iff, not_nonempty_iff_eq_empty, ←sUnion_empty, h.sUnion_eq.symm ]
+--   intro h
+--   rw [ ←Matroid.ground_nonempty_iff, not_nonempty_iff_eq_empty, ←sUnion_empty] at h
+--   refine ⟨h.symm, by grind ⟩
+
+-- lemma coverNumber_zero_iff (P : Matroid α → Set α → Prop) : M.coverNumber P = 0 ↔ M.IsCover P ∅ := by
+--   refine ⟨?_, ?_ ⟩
+--   · intro h
+--     obtain ht | ⟨T, hT, hTe ⟩ := exists_cover M P
+--     · by_contra
+--       rw[ht] at h
+--       simp only [ENat.top_ne_zero] at h
+--     rw [h] at hTe
+--     rwa [← encard_eq_zero.mp hTe  ]
+--   intro h
+--   have := h.coverNumber_le
+--   simp only [encard_empty, nonpos_iff_eq_zero] at this
+--   grind
+
+-- -- lemma coverNumber_le_coverNumber (P Q : Matroid α → Set α → Prop) (M : Matroid α)
+-- --     (hPQ : ∀ X ⊆ M.E, P M X → Q M X) : M.coverNumber Q ≤ M.coverNumber P := by
+-- --   sorry
+
+-- -- lemma coverNumber_congr (P Q : Matroid α → Set α → Prop)
+-- --     (hPQ : ∀ (M : Matroid α) (X : Set α), X ⊆ M.E → (P M X ↔ Q M X)) (M : Matroid α) :
+-- --     M.coverNumber P = M.coverNumber Q := by
+-- --   sorry
+
+-- -- lemma coverNumber_mono_prop (P : Matroid α → Set α → Prop) {M N : Matroid α} (hMN : M.E = N.E)
+-- --     (hMP : ∀ X ⊆ M.E, P N X → P M X) : M.coverNumber P ≤ N.coverNumber P := by
+
+-- --   simp only [coverNumber, le_sInf_iff, mem_image, mem_setOf_eq, forall_exists_index, and_imp,
+-- --     forall_apply_eq_imp_iff₂]
+-- --   refine fun C hC ↦ sInf_le ?_
+-- --   simp only [mem_image, mem_setOf_eq]
+-- --   refine ⟨C, ?_, rfl⟩
+-- --   have := hC.mono_prop (P' := P)
+
+
+-- end General
+
+-- section Rank
+
+-- -- lemma RankPropIsMUProp {k : ℕ∞} : IsMUProp (RankProp α k) (fun M X Y ↦ (M.eRk Y ≤ k + M.eRk X)) := by
+-- --     --use fun M X Y ↦ (M.eRk Y ≤ k + M.eRk X)
+-- --     intro M X Y hXY
+-- --     unfold RankProp at hXY
+-- --     sorry
+
+-- def IsRankCover (M : Matroid α) (k : ℕ∞) (T : Set (Set α )) : Prop :=
+--     M.IsCover (fun M X ↦ M.eRk X ≤ k) T
+
+-- lemma IsRankCover_iff_IsCover (M : Matroid α) (k : ℕ∞) (T : Set (Set α )) :
+--     M.IsRankCover k T ↔ M.IsCover (fun M X ↦ M.eRk X ≤ k) T := Iff.rfl
+
+-- lemma IsRankCover_iff (M : Matroid α) (k : ℕ∞) (T : Set (Set α )) :
+--     M.IsRankCover k T ↔ ⋃₀ T = M.E ∧ (∀ F ∈ T, M.eRk F ≤ k) := by
+--   sorry
+--   --Mathieu
+
+-- lemma IsRankCover_isCover_closure (hcov : M.IsRankCover k T) :
+--     M.IsRankCover k (M.closure '' T) := by
+--   apply hcov.isCover_closure (fun M F hF ↦ ?_)
+--   rwa [(eRk_closure_eq M F) ]
+
+-- lemma IsRankCover.mono_k {k' : ℕ∞} (hcov : M.IsRankCover k T) (hkk' : k ≤ k') :
+--     M.IsRankCover k' T := by
+--   refine ⟨ hcov.sUnion_eq, fun F hF ↦
+--     Std.IsPreorder.le_trans (M.eRk F) k k' (hcov.pProp F hF ) hkk' ⟩
+
+-- lemma IsRankCover_RankPos : M.hasCover_with (fun M X ↦ M.eRk X ≤ 0) ↔ ¬ M.RankPos := by
+--   refine ⟨ ?_, ?_ ⟩
+--   · intro h
+--     refine M.not_rankPos_iff.2 (Matroid.eq_loopyOn_iff_loops.mpr
+--       ⟨Eq.symm (Subset.antisymm ?_ (loops_subset_ground M )) , by simp only ⟩   )
+--     intro e he
+--     obtain ⟨ T, hT ⟩ := h
+--     rw[←hT.sUnion_eq ] at he
+--     obtain ⟨ X, hXt, heX ⟩ := he
+--     exact isLoop_iff.mp (((Matroid.eRk_eq_zero_iff (IsCover.subset_ground hT hXt  )).1
+--       (nonpos_iff_eq_zero.mp (hT.pProp X hXt ))) heX)
+--   intro h
+--   refine ⟨ (singleton '' M.E), IsCover_singleton_Prop ?_ ⟩
+--   intro e he
+--   simp only [nonpos_iff_eq_zero]
+--   refine IsLoop.eRk_eq ?_
+--   rw [M.not_rankPos_iff.1 h]
+--   exact loopyOn_isLoop_iff.mpr he
+
+-- lemma IsRankCover_two [M.Nonempty] (hcov : M.IsRankCover k T) (hk : k < M.eRank ) :
+--     2 ≤ T.encard := by
+--   by_contra hc
+--   simp only [not_le] at hc
+--   have hle : T.encard ≤ 1 := Order.le_of_lt_succ hc
+--   have h1 := ((IsRankCover_iff_IsCover M k T).1 hcov).one_le
+--   have h1 : T.encard = 1 := by grind
+--   obtain ⟨X, hX ⟩ := Set.encard_eq_one.1 h1
+--   have h2 := ((IsRankCover_iff_IsCover M k T).1 hcov).sUnion_eq
+--   rw [hX] at h2
+--   simp only [sUnion_singleton] at h2
+--   have hXT : X ∈ T := by
+--     rw[ hX ]
+--     exact mem_singleton X
+--   have hf := ((IsRankCover_iff_IsCover M k T).1 hcov).pProp X hXT
+--   rw[ h2, ←eRank_def M  ] at hf
+--   grind
+
+
+-- lemma setOf_point_IsRankCover (M : Matroid α) [M.RankPos] : M.IsRankCover 1 {P | M.IsPoint P} := by
+--   refine ⟨subset_antisymm (sUnion_subset fun _ ↦ IsPoint.subset_ground) fun e he ↦ ?_,
+--     by simp +contextual [mem_setOf_eq, IsPoint] ⟩
+--   simp only [mem_sUnion, mem_setOf_eq]
+--   obtain hl | hnl := M.isLoop_or_isNonloop e
+--   · obtain ⟨f, hf⟩ := M.exists_isNonloop
+--     exact ⟨_, hf.closure_isPoint, hl.mem_closure _⟩
+--   exact ⟨_, hnl.closure_isPoint, mem_closure_of_mem _ (by simp) (by simpa)⟩
+
+-- lemma setOf_point_IsCover [hM : M.Loopless] : M.IsRankCover 1 {P | M.IsPoint P} := by
+--   obtain ⟨E, rfl⟩ | h := M.eq_loopyOn_or_rankPos'
+--   · obtain rfl : E = ∅ := by simpa using hM
+--     constructor <;> simp [IsPoint]
+--   exact M.setOf_point_IsRankCover
+
+-- lemma IsRankCover_ground (M : Matroid α) : M.IsRankCover M.eRank ({M.E}) := by
+--   refine ⟨ by simp, fun F a ↦ eRk_le_eRank M F ⟩
+
+-- lemma IsRankCover.nonempty [M.Nonempty] (h : M.IsRankCover k T) : T.Nonempty := by
+--   rw [nonempty_iff_empty_ne]
+--   rintro rfl
+--   simp [IsRankCover_iff, eq_comm, M.ground_nonempty.ne_empty] at h
+
+-- lemma RankPropCover_exists (hk : 1 ≤ k) : M.hasCover_with (fun M X ↦ M.eRk X ≤ k) := by
+--   by_cases hRP : M.RankPos
+--   · refine ⟨{P | M.IsPoint P}, (setOf_point_IsRankCover M ).mono_k hk ⟩
+--   obtain ⟨ T, hT ⟩ := IsRankCover_RankPos.2 hRP
+--   refine ⟨ T, ((IsRankCover_iff_IsCover M 0 T).2 hT).mono_k (ENat.zero_le ) ⟩
+
+-- lemma IsCover.delete (hT : M.IsCover (fun M X ↦ M.eRk X ≤ k) T) (D : Set α) :
+--     (M ＼ D).IsCover (fun M X ↦ M.eRk X ≤ k) ((fun s ↦ s \ D) '' T) := by
+--   refine ⟨ ?_, ?_ ⟩
+--   · refine subset_antisymm (sUnion_subset fun K ↦ ?_) fun e he ↦ ?_
+--     · intro hK
+--       obtain ⟨ X, hX, h ⟩ := hK
+--       rw[ ← h]
+--       exact diff_subset_diff_left (hT.subset_ground hX )
+--     simp only [delete_ground, mem_diff] at he
+--     rw [←hT.sUnion_eq] at he
+--     obtain ⟨X, hX, hXe ⟩ := he.1
+--     have : e ∈ X \ D := mem_diff_of_mem hXe (he.2 )
+--     grind
+--   intro F hF
+--   obtain ⟨ F' ,hF' ,hF2 ⟩ := hF
+--   rw [←hF2]
+--   simp only [delete_eRk_eq', sdiff_idem]
+--   grw [eRk_subset_le M (diff_subset)]
+--   exact hT.pProp F' hF'
+
+-- --Help
+-- lemma coverNumber_eRank [M.Nonempty] : M.coverNumber (fun M' X ↦ M'.eRk X ≤ M.eRank) = 1 := by
+--   have h2 : 1 ≤ M.coverNumber (fun M' X ↦ M'.eRk X ≤ M.eRank ) :=
+--     M.coverNumer_positive (fun M' X ↦ M'.eRk X ≤ M.eRank )
+--   refine h2.antisymm' ?_
+--   simpa using (IsRankCover_ground M).coverNumber_le
+
+-- -- lemma coverNumber_delete_loop (hne : (M ＼ D).Nonempty) (hk : 1 ≤ k) (hD : D ⊆ M.loops ) :
+-- --     M.coverNumber (fun M X ↦ M.eRk X ≤ k) = (M ＼ D).coverNumber (fun M X ↦ M.eRk X ≤ k) := by
+-- --   obtain ⟨T, hT, hTen ⟩ := exists_min_cover (RankPropCover_exists (M := M) hk )
+-- --   have h1 := (hT.delete D ).coverNumber_le
+-- --   grw[encard_image_le (fun s ↦ s \ D) T, hTen ] at h1
+-- --   -- have hkD : (M ＼ D).RankPos := by
+-- --   --   have hh : (M ＼ M.loops).RankPos := Delete_loops_RankPos
+-- --   --   rw [Matroid.rankPos_iff ] at hh
+-- --   --   simp only [delete_isBase_iff] at hh
+-- --   --   refine { empty_not_isBase := ?_ }
+-- --   --   by_contra hc
+-- --   --   exact Ne.elim (fun a ↦ hh ((((Matroid.IsBasis.isBasis_subset (isBasis_ground_iff.mpr hc )
+-- --   --   (empty_subset (M.E \ D) ) (IsLoopEquiv.subset_ground rfl fun ⦃a⦄ a_1 ↦ a_1) ) ).isBasis_subset
+-- --   --     (empty_subset (M.E \ M.loops) ) (diff_subset_diff_right hD ) ).of_delete)) hTen
+-- --   --have : (M ＼ D).Nonempty := rankPos_nonempty
+-- --   obtain ⟨T', hT', hT'en ⟩ := exists_min_cover (RankPropCover_exists (M := (M ＼ D)) hk )
+-- --   have hcov : M.IsCover (fun M X ↦ M.eRk X ≤ k) (M.closure '' T' ) := by
+-- --     refine ⟨ ?_, ?_ ⟩
+-- --     · refine subset_antisymm (sUnion_subset fun K ↦ ?_) fun e he ↦ ?_
+-- --       · simp only [mem_image, forall_exists_index, and_imp]
+-- --         grind
+-- --       by_cases heD : e ∈ D
+-- --       · obtain ⟨ X, hX ⟩ := hT'.nonempty
+-- --         have := (IsLoop.mem_closure (hD heD) X )
+-- --         grind
+-- --       have h2 : e ∈ M.E \ D := mem_diff_of_mem he heD
+-- --       rw[←delete_ground,  ←hT'.sUnion_eq  ] at h2
+-- --       obtain ⟨ X, hX, heX ⟩ := h2
+-- --       have := (mem_closure_of_mem' M heX he )
+-- --       grind
+-- --     intro F hF
+-- --     obtain ⟨F' ,hF', hF2 ⟩ := hF
+-- --     rw[←hF2, eRk_closure_eq M F']
+-- --     have ha := hT'.pProp F' hF'
+-- --     simp only [delete_eRk_eq'] at ha
+-- --     have ha1 : F' \ D = F' := by
+-- --       have := hT'.subset_ground hF'
+-- --       grind
+-- --     rwa [ha1] at ha
+-- --   have h2 := hcov.coverNumber_le
+-- --   grw [encard_image_le M.closure T', hT'en] at h2
+-- --   grind
+
+-- -- lemma coverNumber_contract_loop (hne : (M ＼ D).Nonempty) (hk : 1 ≤ k) (hD : D ⊆ M.loops ) :
+-- --     M.coverNumber (fun M X ↦ M.eRk X ≤ k) = (M ／ D).coverNumber (fun M X ↦ M.eRk X ≤ k) := by
+-- --   rw[contract_eq_delete_of_subset_loops hD]
+-- --   exact coverNumber_delete_loop hne hk hD
+
+-- -- lemma IsRankCover.contract (h : (M ／ X).IsRankCover k T) (hX : X ⊆ M.E)
+-- --     (hXN : (M ／ X).Nonempty) :
+-- --     M.IsRankCover (k + M.eRk X) ((· ∪ X) '' T) := by
+-- --   suffices ∀ F ∈ T, M.eRk (F ∪ X) ≤ k + M.eRk X by
+-- --     simpa [IsRankCover_iff, ← biUnion_distrib_union _ h.nonempty, ← sUnion_eq_biUnion, h.sUnion_eq, hX]
+-- --   exact fun F hFT ↦ by grw [← h.pProp F hFT, ← eRelRk_eq_eRk_contract, eRelRk_add_eRk_eq]
+
+-- -- lemma coverNumber_contract_one {a : ℕ∞} (he : e ∈ M.E) (hel : M.IsNonloop e)
+-- --     (heN : (M／ {e}).Nonempty) :
+-- --     M.coverNumber (fun M X ↦ M.eRk X ≤ (a + 1)) ≤ (M ／ {e}).coverNumber (fun M X ↦ M.eRk X ≤ a)
+-- --     := by
+-- --   refine ENat.forall_natCast_le_iff_le.mp ?_
+-- --   intro b hb
+-- --   unfold coverNumber at hb
+-- --   simp only [le_sInf_iff, mem_image, mem_setOf_eq, forall_exists_index, and_imp,
+-- --     forall_apply_eq_imp_iff₂] at hb
+-- --   unfold coverNumber
+-- --   simp only [le_sInf_iff, mem_image, mem_setOf_eq, forall_exists_index, and_imp,
+-- --     forall_apply_eq_imp_iff₂]
+-- --   intro T hT
+-- --   rw[←IsRankCover_iff_IsCover] at hT
+-- --   have h1 := hT.contract (singleton_subset_iff.mpr he ) heN
+-- --   rw[IsNonloop.eRk_eq hel ] at h1
+-- --   have h2 := hb ((· ∪ {e}) '' T) h1
+-- --   grw[encard_image_le (fun x ↦ x ∪ {e}) T ] at h2
+-- --   exact h2
+
+-- -- lemma exists_cover (M : Matroid α) {k : ℕ∞} (hk : 1 ≤ k) :
+-- --     ∃ T, M.IsCover k T ∧ T.encard = M.coverNumber k := by
+-- --   simpa using csInf_mem <| (M.setOf_cover_nonempty hk).image encard
+
+
+
+-- -- lemma coverNumber_contract {a : ℕ∞} (hX : X ⊆ M.E) :
+-- --     M.coverNumber (a + M.eRk X) ≤ (M ／ X).coverNumber a := by
+-- --   --Mathieu, do you want to do this one?
+-- --   sorry
+
+-- -- def closZ (a : ℕ) (hx : X.Finite ) (hX : X ⊆ M.E)
+-- --     (Y : (M ↾ F).closure '' { Y | Y ⊆ X ∧ M.eRk Y = a} )
+-- --     : ∃ Z :  { Y | Y ⊆ X ∧ M.eRk Y = a}, Y.1 = Z.1 := by
+-- --   have := (mem_image ((M ↾ F).closure) ({ Y | Y ⊆ X ∧ M.eRk Y = a}) Y.1  ).1 Y.2
+-- --   obtain ⟨Y, hY ⟩ := (mem_image ((M ↾ F).closure) ({ Y | Y ⊆ X ∧ M.eRk Y = a}) Y.1  ).1 Y.2
+-- --   sorry
+
+-- -- def IsFlat.restriction_clo (hF : M.IsFlat F) (hY : Y ⊆ F) : M.closure Y = (M ↾ F).closure Y :=
+-- --     by
+-- --   sorry
+
+
+
+-- --Dont need
+-- -- def closZ (a : ℕ)
+-- --     (Z : (M ↾ F).closure '' { Y | Y ⊆ X ∧ M.eRk Y = a} )
+-- --     : ∃ Y :  { Y | Y ⊆ X ∧ M.eRk Y = a}, (M ↾ F).closure Y.1 = Z.1 := by
+-- --   --have := (mem_image ((M ↾ F).closure) ({ Y | Y ⊆ X ∧ M.eRk Y = a}) Y.1  ).1 Y.2
+-- --   obtain ⟨Y, hY, h ⟩ := (mem_image ((M ↾ F).closure) ({ Y | Y ⊆ X ∧ M.eRk Y = a}) Z.1  ).1 Z.2
+-- --   use ⟨Y, hY⟩
+
+-- -- def getI (a : ℕ) (hX : X ⊆ M.E)
+-- --     (Y : { Y | Y ⊆ X ∧ M.eRk Y = a} )
+-- --     : ∃ I : {Y | Y ⊆ X ∧ Y.encard = a}, I.1 ⊆ X ∧ (M.IsBasis I Y.1) ∧ I.1.encard = a := by
+-- --   --have : Y ⊆ M.E := by sorry
+-- --   obtain ⟨I, hIB, hc ⟩ := (M.eq_eRk_iff.1 Y.2.2)
+-- --   have h' :  I ∈ {Y | Y ⊆ X ∧ Y.encard = ↑a} := by
+-- --     refine ⟨LE.le.subset fun ⦃a⦄ a_2 ↦ (Y.2.1 ) (IsBasis.subset hIB  a_2) , hc ⟩
+-- --   use ⟨ I, h' ⟩
+-- --   refine ⟨h'.1, hIB , hc ⟩
+
+-- -- def ranksubsets_Map (a : ℕ) (b : ℕ) (hx : X.Finite ) (hX : X ⊆ M.E) (hF : M.IsFlat F) (hXF : X ⊆ F)
+-- --     : Function.Embedding
+-- --     ((M ↾ F).closure '' { Y | Y ⊆ X ∧ M.eRk Y = a}) {Y | Y ⊆ X ∧ Y.encard = a} :=
+-- -- --have := LE.le.subset fun ⦃a⦄ a_1 ↦ hX (hY.1 a_1)
+-- -- { toFun := fun Z =>
+-- --     ⟨ (Classical.choose (getI a hX (Classical.choose (closZ a Z ))) ).1 ,
+-- --     (Classical.choose (getI a hX (Classical.choose (closZ a Z ))) ).2 ⟩
+-- --   inj' := by
+-- --     intro x y hxy
+-- --     simp only [Subtype.mk.injEq] at hxy
+-- --     have heq : x.1 = y.1 := by
+-- --       rw[ ←(Classical.choose_spec (closZ a x )), ←(Classical.choose_spec (closZ a y )) ]
+-- --       --simp only [mem_setOf_eq, coe_setOf ]
+-- --       rw[←hF.restriction_clo ?_, ←hF.restriction_clo ?_,
+-- --       ←((Classical.choose_spec (getI a hX (Classical.choose (closZ a x ))) ).2.1).closure_eq_closure,
+-- --       ←((Classical.choose_spec (getI a hX (Classical.choose (closZ a y ))) ).2.1).closure_eq_closure,
+-- --       hxy ]
+-- --       --simp only [restrict_closure_eq']
+-- --       --have := (Classical.choose_spec (getI a hX (Classical.choose (closZ a x ))) ).1
+-- --       have := (Classical.choose (closZ a x )).2.1
+-- --       --exact LE.le.subset fun ⦃b⦄ b_2 ↦ hXF (this b_2)
+-- --       --grw[hXF] at this
+-- --       --intro Y hY
+
+-- --       --simp only [mem_setOf_eq, coe_setOf] at this
+
+-- --       sorry
+-- --       · sorry
+-- --     exact SetCoe.ext heq
+-- --     --rw[ ] at hxy
+
+-- --     }
+
+-- lemma set_to_binom_number {a b : ℕ} (X : Set α) (hX : X.encard = b) :
+--     {Y | Y ⊆ X ∧ Y.encard = a}.encard = b.choose a := by
+--   have hXfin : X.Finite := by simp [← encard_lt_top_iff, hX]
+--   set X' := hXfin.toFinset with hX'
+--   have := (ENat.coe_inj).2 <| X'.card_powersetCard a
+--   convert (ENat.coe_inj).2 <| X'.card_powersetCard a
+--   · rw [← encard_coe_eq_coe_finsetCard, ← Finset.coe_injective.encard_image (β := Set α)]
+--     convert rfl
+--     ext S
+--     simp only [mem_image, SetLike.mem_coe, Finset.mem_powersetCard, mem_setOf_eq,
+--       hX', Finite.subset_toFinset]
+--     constructor
+--     · rintro ⟨T, ⟨hTX, rfl⟩, rfl⟩
+--       simpa
+--     intro ⟨hSX, hSa⟩
+--     refine ⟨Finite.toFinset (s := S) ?_, ?_⟩
+--     · simp [← encard_lt_top_iff, hSa]
+--     simp_rw [← ENat.coe_inj, ← hSa, ← Finite.encard_eq_coe_toFinset_card]
+--     simpa
+--   rw [← ENat.coe_inj, ← hX, eq_comm, hXfin.encard_eq_coe_toFinset_card]
+
+-- -- lemma base_isCover {a : ℕ} (hr : M.eRank ≤ a + 1) (ha : 1 ≤ a) (hXfin : X.Finite)
+-- --     --(h : Maximal (fun Y ↦ Y ⊆ M.E ∧ (M ↾ Y).IsFiniteRankUniform (a + 1) Y.encard) X) :
+-- --     (h : MaximalFor (fun x ↦ x ∈ {X | X ⊆ M.E ∧ (M ↾ X).IsFiniteRankUniform (a + 1) X.encard}) encard X) :
+-- --     M.IsRankCover a (M.closure '' {K | K ⊆ X ∧ K.encard = a}) := by
+-- --   refine ⟨?_, ?_⟩
+-- --   · refine subset_antisymm (sUnion_subset fun K ↦ ?_) fun e he ↦ ?_
+-- --     · simp only [mem_image, mem_setOf_eq, forall_exists_index, and_imp]
+-- --       grind
+-- --     obtain ⟨E, hEX, hEunif⟩ := h.prop.2.exists_eq_unifOn
+-- --     obtain rfl : X = E := congr_arg Matroid.E hEunif
+-- --     by_contra! hcon
+-- --     simp only [sUnion_image, mem_setOf_eq, mem_iUnion, exists_prop, not_exists, not_and,
+-- --       and_imp] at hcon
+-- --     have hcon' (Z) (hZ : Z ⊆ X) (hZa : Z.encard ≤ a) : e ∉ M.closure Z := by
+-- --       have haX : a ≤ X.encard := by
+-- --         grw [← M.restrict_ground_eq (R := X), ← eRank_le_encard_ground, h.prop.2.eRank_eq]
+-- --         simp
+-- --       obtain ⟨W, hZW, hWZ, hW⟩ := exists_superset_subset_encard_eq hZ hZa haX
+-- --       exact notMem_subset (M.closure_subset_closure hZW) (hcon W hWZ hW)
+-- --     have heX : e ∉ X := by
+-- --       by_contra hc
+-- --       exact hcon' (singleton e) (singleton_subset_iff.mpr hc )
+-- --         (by simp only [encard_singleton, ENat.one_le_coe, ha ]) (mem_closure_self M e he )
+-- --     --have hwin := h.not_prop_of_ssuperset (t := insert e X) (by grind)
+-- --     have hwin := h.not_prop_of_gt (j := insert e X)
+-- --       (Finite.encard_lt_encard hXfin (ssubset_insert heX ))
+-- --     simp only [mem_setOf_eq, not_and, insert_subset_iff.mpr ⟨he, h.prop.1 ⟩,forall_const ] at hwin
+-- --     --rw [insert_subset_iff , and_iff_right he, and_iff_right h.prop.1] at hwin
+-- --     apply hwin
+-- --     suffices aux : (M ↾ insert e X) = unifOn (insert e X) (a + 1) by
+-- --       rw [aux]
+-- --       apply unifOn_isFiniteRank_uniform
+-- --       grw [h.prop.2.le, ← subset_insert]
+-- --     refine ext_indep rfl fun I (hI : I ⊆ insert e X) ↦ ?_
+-- --     simp only [restrict_indep_iff, hI, and_true, unifOn_indep_iff, Nat.cast_add, Nat.cast_one]
+-- --     refine ⟨fun hIi ↦ by grw [hIi.encard_le_eRank, hr], fun hcard ↦ ?_⟩
+-- --     have hI₀ : M.Indep (I \ {e}) := by
+-- --       have hrestr := (M.restrict_indep_iff (R := X) (I := I \ {e})).1
+-- --       nth_grw 1 [hEunif, unifOn_indep_iff, diff_subset] at hrestr
+-- --       grind
+-- --     by_cases! heI : e ∉ I
+-- --     · rwa [diff_singleton_eq_self heI] at hI₀
+-- --     rw [← insert_diff_self_of_mem heI, hI₀.insert_indep_iff_of_notMem (by grind), mem_diff,
+-- --       and_iff_right he]
+-- --     refine hcon'  _ (by grind) ?_
+-- --     grw [← ENat.add_one_le_add_one_iff, ← hcard, encard_diff_singleton_add_one heI]
+-- --   simp only [mem_image, mem_setOf_eq, forall_exists_index, and_imp]
+-- --   rintro F I hI hcard rfl
+-- --   grw [eRk_closure_eq, eRk_le_encard, hcard]
+
+-- lemma base_isCover {a : ℕ} (hr : M.eRank ≤ a + 1) (ha : 1 ≤ a) (hXfin : X.Finite)
+--     --(h : Maximal (fun Y ↦ Y ⊆ M.E ∧ (M ↾ Y).IsFiniteRankUniform (a + 1) Y.encard) X) :
+--     (h : MaximalFor (fun x ↦ x ∈ {X | X ⊆ M.E ∧ (M ↾ X).IsFiniteRankUniform (a + 1) }) encard X) :
+--     M.IsRankCover a (M.closure '' {K | K ⊆ X ∧ K.encard = a}) := by
+--   refine ⟨?_, ?_⟩
+--   · refine subset_antisymm (sUnion_subset fun K ↦ ?_) fun e he ↦ ?_
+--     · simp only [mem_image, mem_setOf_eq, forall_exists_index, and_imp]
+--       grind
+--     obtain ⟨E, hEX, hEunif⟩ := h.prop.2.exists_eq_unifOn
+--     --obtain rfl : X = E := congr_arg Matroid.E hEunif
+--     by_contra! hcon
+--     simp only [sUnion_image, mem_setOf_eq, mem_iUnion, exists_prop, not_exists, not_and,
+--       and_imp] at hcon
+--     have hcon' (Z) (hZ : Z ⊆ X) (hZa : Z.encard ≤ a) : e ∉ M.closure Z := by
+--       have haX : a ≤ X.encard := by
+--         grw [← M.restrict_ground_eq (R := X), ← eRank_le_encard_ground, h.prop.2.eRank_eq]
+--         simp
+--       obtain ⟨W, hZW, hWZ, hW⟩ := exists_superset_subset_encard_eq hZ hZa haX
+--       exact notMem_subset (M.closure_subset_closure hZW) (hcon W hWZ hW)
+--     have heX : e ∉ X := by
+--       by_contra hc
+--       exact hcon' (singleton e) (singleton_subset_iff.mpr hc )
+--         (by simp only [encard_singleton, ENat.one_le_coe, ha ]) (mem_closure_self M e he )
+--     --have hwin := h.not_prop_of_ssuperset (t := insert e X) (by grind)
+--     have hwin := h.not_prop_of_gt (j := insert e X)
+--       (Finite.encard_lt_encard hXfin (ssubset_insert heX ))
+--     simp only [mem_setOf_eq, not_and, insert_subset_iff.mpr ⟨he, h.prop.1 ⟩,forall_const ] at hwin
+--     --rw [insert_subset_iff , and_iff_right he, and_iff_right h.prop.1] at hwin
+--     apply hwin
+--     suffices aux : (M ↾ insert e X) = unifOn (insert e X) (a + 1) by
+--       rw [aux]
+--       apply unifOn_isFiniteRankUniform
+--       grw [h.prop.2.le , ← subset_insert]
+--       exact encard_le_encard fun ⦃a⦄ a_1 ↦ a_1
+--     refine ext_indep rfl fun I (hI : I ⊆ insert e X) ↦ ?_
+--     simp only [restrict_indep_iff, hI, and_true, unifOn_indep_iff, Nat.cast_add, Nat.cast_one]
+--     refine ⟨fun hIi ↦ by grw [hIi.encard_le_eRank, hr], fun hcard ↦ ?_⟩
+--     have hI₀ : M.Indep (I \ {e}) := by
+--       have hrestr := (M.restrict_indep_iff (R := X) (I := I \ {e})).1
+--       have : I \ {e} ⊆ E  := by
+--         rw [ ←unifOn_ground_eq E (k := a + 1), ← hEX, restrict_ground_eq, diff_subset_iff, singleton_union]
+--         exact LE.le.subset hI
+--       nth_grw 1 [hEX, unifOn_indep_iff, diff_subset] at hrestr
+--       grind
+--     by_cases! heI : e ∉ I
+--     · rwa [diff_singleton_eq_self heI] at hI₀
+--     rw [← insert_diff_self_of_mem heI, hI₀.insert_indep_iff_of_notMem (by grind), mem_diff,
+--       and_iff_right he]
+--     refine hcon'  _ (by grind) ?_
+--     grw [← ENat.add_one_le_add_one_iff, ← hcard, encard_diff_singleton_add_one heI]
+--   simp only [mem_image, mem_setOf_eq, forall_exists_index, and_imp]
+--   rintro F I hI hcard rfl
+--   grw [eRk_closure_eq, eRk_le_encard, hcard]
+
+-- lemma baseCase {a b : ℕ} (ha : 1 ≤ a) (hM : NoUniformMinor M (a + 1) (b + 1))
+--     (hr : M.eRank = a + 1) :
+--     M.coverNumber (fun M X ↦ M.eRk X ≤ a) ≤ Nat.choose b a := by
+--   have : M.RankFinite := M.eRank_ne_top_iff.mp (ENat.ne_top_iff_exists.2
+--       (Exists.intro ((fun x1 x2 ↦ x1 + x2) a 1) (hr.symm)))
+--   by_contra! hcon
+--   obtain ⟨B, hB⟩ := M.exists_isBase
+--   set Unif : Set (Set α) := {X | X ⊆ M.E ∧ (M ↾ X).IsFiniteRankUniform (a + 1) } with h_UnifS
+--   have hne : Unif.Nonempty := by
+--     refine ⟨B, (IsBase.subset_ground hB), ?_, ?_,⟩
+--     · rwa [eRank_restrict, hB.eRk_eq_eRank]
+--     rw [hB.indep.restrict_eq_freeOn]
+--     exact freeOn_uniform B
+--   have hYbound : ∀ Y, Y ∈ Unif → Y.encard < b + 1 := by
+--     intro X hX
+--     by_contra hc
+--     simp only [not_lt] at hc
+--     --have : X ⊆ M.E := by exact hX.1
+--     have h2 : ((unifOn (M ↾ X).E (a + 1)).NoUniformMinor (a + 1) (b + 1)) := by
+--       rw[←hX.2.eq_unifOn ]
+--       exact hM.minor (IsRestriction.isMinor (restrict_isRestriction M X) )
+--     have h3 := unifOn_noUniformMinor_iff.1 h2
+--     grw [← restrict_ground_eq (M := M) (R := X)] at hc
+--     grind
+--     --simp only [mem_setOf_eq] at hX
+--     -- exact hc.not_gt <| hM.lt_of_isoMinor (N := M ↾ X) (b' := X.encard)
+--     --   (restrict_isRestriction _ _ hX.1).isMinor.isoMinor sorry
+--   have hcard : (encard '' Unif).Finite := by
+--     refine ENat.finite_of_sSup_lt_top ?_
+--     refine lt_of_le_of_lt ?_ <| WithTop.natCast_lt_top (b + 1)
+--     simp only [sSup_le_iff, mem_image, forall_exists_index, and_imp]
+--     intro k A hAE h
+--     rw[←h ]
+--     exact Std.le_of_lt (hYbound A ⟨hAE.1, hAE.2 ⟩ )
+--   obtain ⟨X, hX⟩ := Finite.exists_maximalFor' encard _ hcard hne
+--   have hXb : X.encard < b + 1 := hYbound X hX.prop
+--   set Subsets : Set (Set α) := { Y | Y ⊆ X ∧ Y.encard = a} with h_sub
+--   --(Set.encard_le_coe_iff.1 (ENat.lt_coe_add_one_iff.mp hXb )).1
+--   have hiC := base_isCover (Std.le_of_eq hr ) ha
+--       ((Set.encard_le_coe_iff.1 (ENat.lt_coe_add_one_iff.mp hXb )).1) hX
+--   --have hiC : M.IsCover (fun M X ↦ M.eRk X ≤ a) (M.closure '' Subsets) := by base_isCover
+--   obtain ⟨x, hx ⟩ := ENat.ne_top_iff_exists.1 (LT.lt.ne_top hXb )
+--   rw[←hx] at hXb
+--   grw [hiC.coverNumber_le, Set.encard_image_le, (set_to_binom_number) X hx.symm,
+--     (Nat.choose_le_choose a (Nat.le_of_lt_succ (ENat.coe_lt_coe.mp hXb )))] at hcon
+--   simp only [lt_self_iff_false] at hcon
+
+-- lemma coverNumber_rank_Frombase {a b : ℕ} (ha : 1 ≤ a)
+--     (hM : NoUniformMinor M ( a + 1 ) (b + 1)) :
+--     M.coverNumber (fun M X ↦ M.eRk X ≤ a) ≤
+--     (Nat.choose b a) * M.coverNumber (fun M X ↦ M.eRk X ≤ (a + 1)) := by
+--   sorry
+
+-- lemma coverNumber_Bound {M : Matroid α} [M.RankPos] {a b : ℕ} {n : ℕ∞} (ha : a ≠ 0) (hb : a ≤ b)
+--     (hM : NoUniformMinor M ( a + 1 ) (b + 1)) (hn : M.eRank = a + n) :
+--     M.coverNumber (fun M X ↦ M.eRk X ≤ a) ≤ (Nat.choose b a)^(M.eRank - a) := by
+--   obtain htop | hfin := eq_or_ne M.eRank ⊤
+--   · grw [htop, ENat.top_sub_coe, ENat.epow_top, ← le_top]
+--     obtain rfl | hlt := hb.eq_or_lt
+--     · simp [noUniformMinor_self_iff, htop] at hM
+--     rw [← ENat.coe_one, ENat.coe_lt_coe]
+--     suffices b.choose a ≠ 0 ∧ b.choose a ≠ 1 by lia
+--     exact ⟨(Nat.choose_pos hlt.le).ne.symm, by simp [Nat.choose_eq_one_iff, hlt.ne.symm, ha]⟩
+--   by_cases h0 : n = 0
+--   · -- When M.eRank = a, you can cover with (M.E). This is a lemma somewhere
+--     sorry
+--   --Now you can assume n ≠ 0 and n - 1 makes sense
+--   obtain ⟨e, heC⟩ : ∃ e, M.IsNonloop e := exists_isNonloop M
+--   have h' : (M ／ {e}).eRank < M.eRank := by sorry
+--   have hRP : ( M ／ {e}).RankPos := by sorry --I think here you need n ≠ 0
+--   have hM' : NoUniformMinor ( M ／ {e}) ( a + 1 ) (b + 1) := by sorry
+--   have hn' : (M ／ {e}).eRank = a + (n - 1) := by sorry
+--   have ih := coverNumber_Bound (M := M ／ {e}) (a := a) (b := b) ha hb hM' (n := n - 1)
+--   sorry
+-- termination_by M.eRank
+
+--   -- suffices hn : ∀ n : ℕ, M.eRank = n + a + 1 →
+--   --     M.coverNumber (fun M X ↦ M.eRk X ≤ a) ≤ (Nat.choose b a)^(n + 1 )
+--   -- ·
+--   --   sorry
+--   -- intro n hn
+--   -- induction n generalizing M with
+--   -- | zero => sorry
+--   -- | succ n IH => sorry
+
+-- -- -- change `ha` to `a ≠ 0`.
+-- -- lemma coverNumber_Bound_contract [M.RankFinite] {a b : ℕ} (ha : 1 ≤ a)
+-- --     (hM : NoUniformMinor M ( a + 1 ) (b + 1)) (hC : C ⊂ M.E)  :
+-- --     M.coverNumber (fun M X ↦ M.eRk X ≤ a) ≤
+-- --     (Nat.choose b a)^(M.eRk C ) * (M／C).coverNumber (fun M X ↦ M.eRk X ≤ a) := by
+-- --   suffices hn : ∀ n : ℕ, n = M.eRk C →  M.coverNumber (fun M X ↦ M.eRk X ≤ a) ≤
+-- --       (Nat.choose b a)^n * (M／C).coverNumber (fun M X ↦ M.eRk X ≤ a)
+-- --   · obtain ⟨ n, hh ⟩ := ENat.ne_top_iff_exists.1 ( eRk_ne_top (M := M) (X := C))
+-- --     rw[←hh]
+-- --     exact le_of_eq_of_le rfl (hn n hh)
+-- --   intro n hn
+-- --   induction n generalizing M C with
+-- --   | zero =>
+-- --     simp only [pow_zero, one_mul]
+-- --     rw [coverNumber_contract_loop ((ground_nonempty_iff (M ＼ C)).mp (nonempty_of_ssubset hC ) )
+-- --       (ENat.one_le_coe.mpr ha ) ((eRk_eq_zero_iff (subset_of_ssubset hC)).1 hn.symm )]
+-- --   | succ n IH =>
+-- --   grw[coverNumber_rank_Frombase ha hM ]
+-- --   have hresP : (M ↾ C).RankPos :=
+-- --     (eRank_ne_zero_iff (M ↾ C)).mp <| by simp [eRank_restrict, ne_eq, ← hn]
+
+-- --   obtain ⟨e, heC ⟩ := exists_isNonloop (M ↾ C)
+-- --   obtain ⟨heC1, heC2 ⟩ := restrict_isNonloop_iff.1 heC
+-- --   have heN : (M／ {e}).Nonempty := by
+-- --     rw[←(M／ {e}).ground_nonempty_iff, contract_ground]
+-- --     exact (Set.nonempty_of_ssubset (by grind ) )
+-- --   grw[ coverNumber_contract_one (heC1.mem_ground ) heC1 heN]
+-- --   have hn1 : (M／ {e}).eRk (C \ {e}) = n := by
+-- --     have hrelrk := IsNonloop.eRelRk_add_one_eq heC1 (C \ {e})
+-- --     simp only [insert_diff_singleton, insert_eq_of_mem heC2, ←hn, Nat.cast_add, Nat.cast_one,
+-- --       ne_eq, ENat.one_ne_top, not_false_eq_true,
+-- --       add_left_inj_of_ne_top] at hrelrk
+-- --     rwa [eRelRk.eq_1] at hrelrk
+-- --   have hsub1 : (C \ {e}) ⊂ (M／ {e}).E := by
+-- --     simp only [contract_ground]
+-- --     refine Set.ssubset_iff_subset_ne.mpr ⟨diff_subset_diff_left (subset_of_ssubset hC), ?_ ⟩
+-- --     by_contra hc
+-- --     have h : C = M.E := by
+-- --       rw [←insert_diff_self_of_mem heC2, ←insert_diff_self_of_mem heC1.mem_ground, hc]
+-- --     have hCE : C ≠ M.E := by exact Std.ne_of_lt hC
+-- --     rw [h] at hCE
+-- --     exact false_of_ne hCE
+-- --   grw[ IH (hM.minor (contract_isMinor M {e} )) hsub1 hn1.symm ]
+-- --   simp only [contract_contract, union_diff_self, singleton_union, ge_iff_le, insert_eq_of_mem heC2,
+-- --     ←mul_assoc ]
+-- --   nth_rw 1 [ ←ENat.epow_one (x := ↑(b.choose a)), ←ENat.epow_natCast,
+-- --     ←ENat.epow_add (x :=  ↑(b.choose a)) (y := 1) (z := n ), ←ENat.coe_one, ←ENat.coe_add,
+-- --     ENat.epow_natCast, add_comm ]
+
+
+-- -- change `ha` to `a ≠ 0`.
+-- lemma coverNumber_Bound_contract {M : Matroid α} {C : Set α} {a b : ℕ} (ha : a ≠ 0) (hb : a ≤ b)
+--     (hM : NoUniformMinor M (a + 1) (b + 1)) (hC : C ⊂ M.E)  :
+--     M.coverNumber (fun M X ↦ M.eRk X ≤ a) ≤
+--     (Nat.choose b a)^(M.eRk C) * (M ／ C).coverNumber (fun M X ↦ M.eRk X ≤ a) := by
+--   obtain htop | hlt := eq_or_ne (M.eRk C) ⊤
+--   · grw [htop, ENat.epow_top, ENat.top_mul, ← le_top ]
+--     · have heN : (M／ C).Nonempty := by
+--         rw[←(M／ C).ground_nonempty_iff, contract_ground]
+--         exact (Set.nonempty_of_ssubset (by grind ) )
+--       exact ENat.one_le_iff_ne_zero.mp (coverNumer_positive (fun M X ↦ M.eRk X ≤ a) )
+--     obtain rfl | hlt := hb.eq_or_lt
+--     · simp [noUniformMinor_self_iff] at hM
+--       grw [ ←eRk_le_eRank M C, htop ] at hM
+--       simp only [not_top_lt] at hM
+--     rw [← ENat.coe_one, ENat.coe_lt_coe]
+--     suffices b.choose a ≠ 0 ∧ b.choose a ≠ 1 by lia
+--     exact ⟨(Nat.choose_pos hlt.le).ne.symm, by simp [Nat.choose_eq_one_iff, hlt.ne.symm, ha] ⟩
+--   have hresP : (M ↾ C).RankPos := sorry
+--     -- (eRank_ne_zero_iff (M ↾ C)).mp <| by simp [eRank_restrict, ne_eq, ← hn]
+--   obtain ⟨e, heC⟩ : ∃ e, (M ↾ C).IsNonloop e := exists_isNonloop (M ↾ C)
+--   rw [restrict_isNonloop_iff] at heC
+--   -- have hrelrk := IsNonloop.eRelRk_add_one_eq heC.1 (C \ {e})
+--   -- simp only [insert_diff_singleton, insert_eq_of_mem heC.2] at hrelrk
+--   have h' : (M ／ {e}).eRk (C \ {e}) < M.eRk C := by
+--     have hrelrk := IsNonloop.eRelRk_add_one_eq heC.1 (C \ {e})
+--     simp only [insert_diff_singleton, insert_eq_of_mem heC.2] at hrelrk
+--     rw [ ←hrelrk, eRelRk.eq_1 ]
+--     simp only [ENat.lt_add_left_iff, ne_eq, eRk_eq_top_iff, IsRkFinite.diff_singleton_iff, not_not,
+--       one_ne_zero, not_false_eq_true, and_true]
+--     rw [ IsRkFinite ]
+--     refine eRank_lt_top_iff.mp ?_
+--     grw [eRank_restrict, eRk_contract_le_eRk M {e} C]
+--     exact Ne.lt_top' (id (Ne.symm hlt))
+--   have hsub1 : (C \ {e}) ⊂ (M／ {e}).E := by
+--     simp only [contract_ground]
+--     refine Set.ssubset_iff_subset_ne.mpr ⟨diff_subset_diff_left (subset_of_ssubset hC), ?_ ⟩
+--     by_contra hc
+--     have h : C = M.E := by
+--       rw [←insert_diff_self_of_mem heC.2, ←insert_diff_self_of_mem heC.1.mem_ground, hc]
+--     grind
+--   have heN : (M／ {e}).Nonempty := by
+--     rw[←(M／ {e}).ground_nonempty_iff, contract_ground]
+--     exact (Set.nonempty_of_ssubset (by grind ) )
+--   have : 1 ≤ a := by exact Nat.one_le_iff_ne_zero.mpr ha
+--   have ih := coverNumber_Bound_contract (M := M ／ {e}) (C := C \ {e}) (a := a) (b := b) ha
+--     hb (hM.minor (contract_isMinor M {e} )) hsub1
+--   grw [coverNumber_rank_Frombase (Nat.one_le_iff_ne_zero.mpr ha) hM, coverNumber_contract_one (heC.1.mem_ground ) heC.1 heN, ih ]
+--   simp only [contract_contract, union_diff_self, singleton_union, ge_iff_le, insert_eq_of_mem heC.2,
+--     ←mul_assoc]
+--   nth_rw 1 [←eRelRk.eq_1, ←ENat.epow_one (x := ↑(b.choose a)),
+--     ←ENat.epow_add (x :=  ↑(b.choose a)) (y := 1) (z := (M.eRelRk {e} (C \ {e})) ),
+--     ←add_comm (a := (M.eRelRk {e} (C \ {e}))) (b:= 1 ), (heC.1).eRelRk_add_one_eq, insert_diff_singleton, insert_eq_of_mem heC.2 ]
+
+-- termination_by M.eRk C
+
+
+-- end Rank
+
+-- section NonSpanning
+
+-- lemma NonSpanning_to_RankCover [M.RankFinite] (hM : 2 ≤ M.eRank) :
+--     M.IsCover Matroid.Nonspanning T ↔ M.IsRankCover (M.eRank - 1) T := by
+--   refine ⟨?_, ?_ ⟩
+--   · intro h
+--     refine ⟨ h.sUnion_eq, ?_ ⟩
+--     intro F hF
+--     by_contra hc
+--     simp only [not_le] at hc
+--     have : M.eRank ≤ M.eRk F := by
+--       have : M.eRank - 1 + 1 ≤  M.eRk F := by exact Order.add_one_le_of_lt hc
+--       sorry
+--     sorry
+--   sorry
+
+-- lemma NonSpaning_le_two [M.Nonempty] (hle : M.eRank ≤ 1) :
+--     ⊤ ≤ M.coverNumber (Matroid.Nonspanning) := by
+--   obtain hT | ⟨T, hT1, hT2 ⟩  := M.exists_cover (Matroid.Nonspanning)
+--   · rw[ hT ]
+--   by_contra hc
+--   have : M.RankFinite := by
+--     refine eRank_lt_top_iff.mp ?_
+--     grw[hle]
+--     exact ENat.one_lt_top
+--   have hu := hT1.sUnion_eq
+--   have hl : ∀ T1 ∈ T, T1 ⊆ M.loops := by
+--     intro T1 hT'
+--     have h1 : M.eRk T1 < M.eRank := Nonspanning.eRk_lt (hT1.pProp T1 hT' )
+--     grw [hle] at h1
+--     simp only [ENat.lt_one_iff] at h1
+--     exact (M.eRk_eq_zero_iff (X := T1) (hX := by grind)).1 h1
+--   have hs : M.E ⊆ M.loops := by
+--     rw [←hT1.sUnion_eq]
+--     exact sUnion_subset hl
+--   obtain ⟨T', hT' ⟩ := hT1.nonempty
+--   have h2 : M.E ⊆ M.closure T' := by
+--     grw [hs]
+--     exact loops_subset_closure M T'
+--   exact Ne.elim (fun a ↦ ((hT1.pProp T' hT').not_spanning) ((spanning_iff_ground_subset_closure
+--     (hT1.subset_ground hT') ).2 h2)) hT2
+
+
+-- lemma Non_spanning_singleton (he : e ∈ M.E) (hM : 2 ≤ M.eRank) : M.Nonspanning {e} := by
+--     by_contra hc
+--     have h1 : M.eRank ≤ 1 := by
+--       rw [not_nonspanning_iff] at hc
+--       rw [←hc.eRk_eq]
+--       simp only [eRk_singleton_le]
+--     grw [←hM] at h1
+--     simp only [ENat.not_ofNat_le_one] at h1
+
+-- lemma IsCover_singleton_NonSpanning (hM : 2 ≤ M.eRank) :
+--     M.IsCover (Matroid.Nonspanning) (singleton '' M.E) := by
+--   exact IsCover_singleton_Prop (fun e he ↦ Non_spanning_singleton he hM)
+
+-- lemma IsCover_singleton_le_NonSpanning (hM : 2 ≤ M.eRank) :
+--     M.coverNumber (Matroid.Nonspanning) ≤ M.E.encard := by
+--   exact IsCover_singleton_le (fun e he ↦ Non_spanning_singleton he hM)
+
+-- lemma NonSpaning_cover_exists (hM : 2 ≤ M.eRank) : M.hasCover_with Matroid.Nonspanning := by
+--   refine ⟨(singleton '' M.E), IsCover_singleton_NonSpanning hM ⟩
+
+-- lemma IsNonSpaningCover_contract (h : (M ／ X).IsCover (Matroid.Nonspanning) T)
+--     (hX : X ⊆ M.E) (hXN : (M ／ X).Nonempty) :
+--     M.IsCover (Matroid.Nonspanning) ((· ∪ X) '' T) := by
+--   apply h.contract hX hXN
+--   intro Y hC
+--   refine ⟨ ?_, union_subset (by have := hC.subset_ground; grind ) hX  ⟩
+--   · by_contra hc
+--     have hcc : (M ／ X).Spanning Y := by
+--       have h1 := hc.contract X
+--       simp only [union_diff_right] at h1
+--       exact h1.superset (diff_subset (s := Y) (t := X)) (hC.subset_ground)
+--     rw [←not_spanning_iff hcc.subset_ground ] at hC
+--     exact (iff_false_intro hC).mp hcc
+
+-- lemma NonSpanningNumber_contract (hX : X ⊆ M.E) (hne : (M ／ X).Nonempty) :
+--     M.coverNumber Matroid.Nonspanning ≤ (M ／ X).coverNumber Matroid.Nonspanning := by
+--   obtain hT | ⟨T, hT, hTe ⟩ := (M ／ X).exists_cover (Matroid.Nonspanning)
+--   · rw [hT]
+--     exact OrderTop.le_top (M.coverNumber Nonspanning)
+--   rw [← hTe]
+--   exact
+--     Std.IsPreorder.le_trans (M.coverNumber Nonspanning) ((fun x ↦ x ∪ X) '' T).encard T.encard
+--       ((IsNonSpaningCover_contract hT hX hne).coverNumber_le)
+--       (encard_image_le (fun x ↦ x ∪ X) T )
+
+-- lemma NonSpanningNumber_set_closure (hY : Y ⊆ M.closure X) (hX : X ⊆ M.E) :
+--     (M ↾ X).coverNumber Nonspanning  ≤ (M ↾ (X ∪ Y)).coverNumber Nonspanning := by
+--   obtain hT | ⟨T, hT, hTe ⟩ := (M ↾ (X ∪ Y)).exists_cover (Matroid.Nonspanning)
+--   · rw [hT]
+--     exact OrderTop.le_top ((M ↾ X).coverNumber Nonspanning)
+--   rw[←hTe]
+--   have hcov : (M ↾ X).IsCover (Matroid.Nonspanning) ((fun x ↦ x ∩ X) '' T) := by
+--     refine ⟨?_, ?_ ⟩
+--     · refine subset_antisymm (sUnion_subset fun K ↦ ?_) fun e he ↦ ?_
+--       · intro hK
+--         obtain ⟨K', hK'T, hK' ⟩ := hK
+--         rw [← hK']
+--         grind
+--       have h1 := hT.sUnion_eq
+--       simp only [restrict_ground_eq] at h1
+--       simp only [restrict_ground_eq] at he
+--       have : e ∈  ⋃₀ T := by grind
+--       obtain ⟨ T', hT', heT' ⟩ := this
+--       have : e ∈ T' ∩ X := by grind
+--       grind
+--     intro F hF
+--     obtain ⟨F', hF', hhF' ⟩ := hF
+--     simp only at hhF'
+--     rw [← hhF']
+--     by_contra hc
+--     rw [not_nonspanning_iff, restrict_spanning_iff (by grind)] at hc
+--     have hcc : X ∪ Y ⊆ M.closure F' := union_subset (LE.le.subset fun ⦃a⦄ a_1 ↦
+--       (closure_subset_closure M (inter_subset_left )) (hc a_1)) ( LE.le.subset fun ⦃a⦄ a_1 ↦
+--       (closure_subset_closure M (inter_subset_left )) ((LE.le.subset fun ⦃a⦄ a_1 ↦
+--       (closure_subset_closure_of_subset_closure hc ) (hY a_1) ) a_1))
+--     rw [←restrict_spanning_iff (hR := by grind), ←not_nonspanning_iff (by grind)  ] at hcc
+--     exact Ne.elim (fun a ↦ hcc (hT.pProp F' hF')) hTe
+--     exact LE.le.subset (hT.subset_ground hF')
+--   grw [hcov.coverNumber_le ]
+--   exact encard_image_le (fun x ↦ x ∩ X) T
+
+
+
+-- -- lemma NonSpaningNumber_delete_loop (hne : (M ＼ D).Nonempty) (hk : 1 ≤ k) (hD : D ⊆ M.loops ) :
+-- --     M.coverNumber (fun M X ↦ M.eRk X ≤ k) = (M ＼ D).coverNumber (fun M X ↦ M.eRk X ≤ k) := by
+
+-- --   sorry
+--   -- obtain ⟨T, hT, hTen ⟩ := exists_min_cover (RankPropCover_exists (M := M) hk )
+--   -- have h1 := (hT.delete D ).coverNumber_le
+--   -- grw[encard_image_le (fun s ↦ s \ D) T, hTen ] at h1
+--   -- obtain ⟨T', hT', hT'en ⟩ := exists_min_cover (RankPropCover_exists (M := (M ＼ D)) hk )
+--   -- have hcov : M.IsCover (fun M X ↦ M.eRk X ≤ k) (M.closure '' T' ) := by
+--   --   refine ⟨ ?_, ?_ ⟩
+--   --   · refine subset_antisymm (sUnion_subset fun K ↦ ?_) fun e he ↦ ?_
+--   --     · simp only [mem_image, forall_exists_index, and_imp]
+--   --       grind
+--   --     by_cases heD : e ∈ D
+--   --     · obtain ⟨ X, hX ⟩ := hT'.nonempty
+--   --       have := (IsLoop.mem_closure (hD heD) X )
+--   --       grind
+--   --     have h2 : e ∈ M.E \ D := mem_diff_of_mem he heD
+--   --     rw[←delete_ground,  ←hT'.sUnion_eq  ] at h2
+--   --     obtain ⟨ X, hX, heX ⟩ := h2
+--   --     have := (mem_closure_of_mem' M heX he )
+--   --     grind
+--   --   intro F hF
+--   --   obtain ⟨F' ,hF', hF2 ⟩ := hF
+--   --   rw[←hF2, eRk_closure_eq M F']
+--   --   have ha := hT'.pProp F' hF'
+--   --   simp only [delete_eRk_eq'] at ha
+--   --   have ha1 : F' \ D = F' := by
+--   --     have := hT'.subset_ground hF'
+--   --     grind
+--   --   rwa [ha1] at ha
+--   -- have h2 := hcov.coverNumber_le
+--   -- grw [encard_image_le M.closure T', hT'en] at h2
+--   -- grind
+
+-- -- lemma NonSpaningNumber_contract_loop (hne : (M ＼ D).Nonempty) (hk : 1 ≤ k) (hD : D ⊆ M.loops ) :
+-- --     M.coverNumber (fun M X ↦ M.eRk X ≤ k) = (M ／ D).coverNumber (fun M X ↦ M.eRk X ≤ k) := by
+-- --   rw[contract_eq_delete_of_subset_loops hD]
+-- --   exact coverNumber_delete_loop hne hk hD
+
+
+
+
+-- end NonSpanning
 
 
 
