Matroid/Extremal/Thickness.lean
@@ -1,5 +1,4 @@
 import Matroid.Extremal.Covers
-import Matroid.Order.Quotient
 
 set_option linter.style.longLine false
 
@@ -7,63 +6,55 @@ variable {α : Type*} {M N M' : Matroid α} {I F X Y F' F₀ F₁ F₂ P L H H�
   {e f : α} {l r : ℕ} {a k d : ℕ∞} {T : Set (Set α)} {ι : Type*} {i j : ι}
   {P P' : Matroid α → Set α → Prop}
 
-
 open Set
 namespace Matroid
 
 section Thick
 
-def IsThick (M : Matroid α) (d : ℕ∞) : Prop := d ≤ M.coverNumber Matroid.Nonspanning
+def IsThick (M : Matroid α) (X : Set α) (d : ℕ∞) : Prop := d ≤ X.coverNumber (M ↾ X).Nonspanning
 
-lemma IsThick_iff (M : Matroid α) (d : ℕ∞) :
-    M.IsThick d ↔ d ≤ M.coverNumber Matroid.Nonspanning := Eq.to_iff rfl
+lemma IsThick_iff {M : Matroid α} {X : Set α} {d : ℕ∞} :
+    M.IsThick X d ↔ d ≤ X.coverNumber (M ↾ X).Nonspanning := Eq.to_iff rfl
 
-lemma IsThick_iff' (M : Matroid α) (d : ℕ∞) :
-    M.IsThick d ↔ ∀ T, M.IsCover Matroid.Nonspanning T → d ≤ T.encard := by
+lemma IsThick_iff' {M : Matroid α} {X : Set α} {d : ℕ∞} :
+    M.IsThick X d ↔ ∀ T, NonSpanningCover M T X → d ≤ T.encard := by
   refine ⟨?_, ?_ ⟩
   · intro h T hT
+
     sorry
   sorry
 
 
+-- def IsThick_set (M : Matroid α) (X : Set α ) (d : ℕ∞) : Prop :=
+--     (M ↾ X).IsThick d
 
-def IsThickSet (M : Matroid α) (X : Set α ) (d : ℕ∞) : Prop :=
-    (M ↾ X).IsThick d
+-- lemma IsThick_set_iff (M : Matroid α) (X : Set α ) (d : ℕ∞) :
+--     M.IsThick_set X d ↔ d ≤ (M ↾ X).coverNumber Matroid.Nonspanning := by
+--   sorry
 
-lemma isThickSet_iff (M : Matroid α) (X : Set α ) (d : ℕ∞) :
-    M.IsThickSet X d ↔ d ≤ (M ↾ X).coverNumber Matroid.Nonspanning := by
-  sorry
-
-lemma IsThick.of_isQuotient {M N : Matroid α} (hM : M.IsThick d) (hNM : N ≤q M) : N.IsThick d := by
-
-  rw [IsThick_iff] at ⊢ hM
-  grw [hM, coverNumber_le_coverNumber (fun _ X ↦ N.Nonspanning X) Matroid.Nonspanning M ?_]
-
-  -- apply coverNumber_mono
-
-
-lemma IsThick_two (M : Matroid α) [M.Nonempty] : M.IsThick 2 := by
-  rw [M.IsThick_iff 2]
-  obtain ht | ⟨T, hT, hTe ⟩ := exists_cover M Matroid.Nonspanning
+lemma IsThick_two (M : Matroid α) (hX: X.Nonempty) : M.IsThick X 2 := by
+  rw [IsThick_iff ]
+  obtain ht | ⟨T, hT, hTe ⟩ := X.exists_cover (M ↾ X).Nonspanning
   · rw [ ht]
     simp only [le_top]
   rw [← hTe ]
   by_contra hc
-  obtain ⟨X, hX ⟩ := encard_eq_one.mp ((ENat.one_le_iff_ne_zero.mpr (encard_ne_zero.mpr
-    ( hT.nonempty ))).antisymm' (Order.le_of_lt_succ (Std.not_le.mp hc ) ) )
-  have hc1 : M.Spanning X := by
-    rw [← sUnion_singleton (s := X), ←hX, hT.sUnion_eq]
-    refine ⟨ by simp only [closure_ground], by simp only [subset_refl] ⟩
-  exact Ne.elim (fun a ↦ (hT.pProp X ( by rw [hX]; exact mem_singleton X )).not_spanning  hc1) hTe
+  obtain ⟨Y, hY ⟩ := encard_eq_one.mp ((ENat.one_le_iff_ne_zero.mpr (encard_ne_zero.mpr
+    ( hT.nonempty hX ))).antisymm' (Order.le_of_lt_succ (Std.not_le.mp hc ) ) )
+  have hc1 : (M ↾ X).Spanning Y := by
+    rw [← sUnion_singleton (s := Y), ←hY, hT.sUnion_eq]
+    refine ⟨ ?_, IsLoopEquiv.subset_ground rfl fun ⦃a⦄ a_1 ↦ a_1  ⟩
+    nth_rw 2 [← restrict_ground_eq (M := M) (R := X)]
+    simp only [closure_ground]
+    --refine ⟨ by simp only [closure_ground], by simp only [subset_refl] ⟩
+  exact Ne.elim (fun a ↦ (hT.pProp Y ( by rw [hY]; exact mem_singleton Y )).not_spanning  hc1) hTe
 
-lemma IsThick.mono {d' : ℕ∞} (hTd : M.IsThick d ) (hd : d' ≤ d ) : M.IsThick d' := by sorry
+lemma IsThick.mono {d' : ℕ∞} (hTd : M.IsThick X d ) (hd : d' ≤ d ) : M.IsThick X d' := by sorry
 
-lemma IsThick_ground_set (M : Matroid α) (d : ℕ∞) : M.IsThickSet M.E d ↔ M.IsThick d := by sorry
-
-lemma IsThick_set.Minor_mon (hTXd : M.IsThickSet X d) (hNM : N ≤m M ) ( hX : X ⊆ N.E )
-    (hXne : X.Nonempty) : N.IsThickSet X d := by
-
-  rw [N.isThickSet_iff X d]
+lemma IsThick_set.Minor_mon (hTXd : M.IsThick X d) (hNM : N ≤m M ) ( hX : X ⊆ N.E )
+    (hXne : (M ↾ X ).Nonempty) :
+    N.IsThick X d := by
+  rw [N.IsThick_iff ]
   obtain ⟨C, D, hC, hD, hDC, hrw ⟩ := hNM.exists_contract_indep_delete_coindep
   have hDX : Disjoint D X := by grind
   have hCX : Disjoint C X := by grind
@@ -73,30 +64,29 @@ lemma IsThick_set.Minor_mon (hTXd : M.IsThickSet X d) (hNM : N ≤m M ) ( hX : X
     simp only [contract_ground, restrict_ground_eq, union_diff_right]
     have : (X \ C).Nonempty := by
       rw [ Disjoint.sdiff_eq_right hCX ]
-      assumption
+      rwa [←(M ↾ X).ground_nonempty_iff, restrict_ground_eq] at hXne
     refine nonempty_of_not_subset ?_
     have : ¬X ⊆ C := by
       exact not_subset.mpr this
     grind
+  sorry
   -- Peter?
-  have hP : (M ／ C ↾ X) = (M ／ (C ∩ M.closure X) ↾ X) := sorry
+  -- have hP : (M ／ C ↾ X) = (M ／ (C ∩ M.closure X) ↾ X) := by sorry
+  -- have hCX' : Disjoint (C ∩ M.closure X) X := by grind
+  -- grw [hrw, delete_restrict_eq_restrict (M ／ C) hDX, hP,
+  --   M.contract_restrict_eq_restrict_contract hCX',
+  --   ←NonSpanningNumber_contract hg3 hne, ← NonSpanningNumber_set_closure (inter_subset_right)
+  --   (by grind) ]
+  -- exact (IsThick_set_iff M X d).mp hTXd
 
-  have hCX' : Disjoint (C ∩ M.closure X) X := by grind
-  grw [hrw, delete_restrict_eq_restrict (M ／ C) hDX, hP,
-    M.contract_restrict_eq_restrict_contract hCX',
-    ←NonSpanningNumber_contract hg3 hne, ← NonSpanningNumber_set_closure (inter_subset_right)
-    (by grind) ]
-  exact (isThick_set_iff M X d).mp hTXd
-
-lemma IsThick.Contract_mon (hTXd : M.IsThick d) (hC : C ⊆ M.E ) (hne : (M ／ C).Nonempty)
-    : (M ／ C).IsThick d := by
-  grw [IsThick_iff, ←NonSpanningNumber_contract hC hne  ]
-  exact (IsThick_iff M d).mp hTXd
+lemma IsThick.Contract_mon (hTXd : M.IsThick X d) (hC : C ⊆ X ) (hne : (X \ C).Nonempty)
+    : (M ／ C).IsThick (X \ C) d := by
+  grw [IsThick_iff, ←NonSpanningNumber_contract_subset hC hne  ]
+  exact (IsThick_iff ).mp hTXd
 
 
 --Need Approval
-lemma exists_minor_encard (M : Matroid α) (hr : a ≤ M.eRank) :
-    ∃ X, X ⊆ M.E ∧ (M ／ X).eRank = a := by
+lemma exists_minor_encard (M : Matroid α) (hr : a ≤ M.eRank ) : ∃ X, X ⊆ M.E ∧ ( M ／ X).eRank = a := by
   obtain ⟨B, hB ⟩ := M.exists_isBase
   grw [← hB.encard_eq_eRank] at hr
   have ⟨Y, hYB, hYen ⟩ : ∃ Y, Y ⊆ B ∧ Y.encard = a := exists_subset_encard_eq hr
@@ -107,18 +97,35 @@ lemma exists_minor_encard (M : Matroid α) (hr : a ≤ M.eRank) :
     (isBasis_ground_iff.mpr hB) (by grind) ]
   simpa [sdiff_sdiff_right_self, inf_eq_inter, inter_eq_self_of_subset_right hYB ]
 
-lemma thick_Bound {M : Matroid α} [M.RankPos] {a b : ℕ} (ha : a ≠ 0) (hb : a ≤ b)
-    (hM : NoUniformMinor M (a + 1) (b + 1)) (ht : M.IsThick (Nat.choose b a)) : M.eRank ≤ a := by
+lemma exists_minor_encard_eRk (M : Matroid α) (X : Set α) (hr : a ≤ M.eRk X ) :
+    ∃ C, C ⊆ X ∧ ( M ／ C).eRk (X \ C) = a := by
+  sorry
+
+lemma thick_Bound {M : Matroid α} [M.RankPos] {a b : ℕ} (ha : a ≠ 0) (hb : a ≤ b) (hX : X ⊆ M.E)
+    (hM : NoUniformMinor M ( a + 1 ) (b + 1)) (ht : M.IsThick X (Nat.choose b a)) :
+    M.eRk X ≤ a := by
   by_contra hc
   simp only [not_le] at hc
-  wlog hlt : M.eRank = a + 1 generalizing M with aux
-  · obtain ⟨X, hX, hXeRK ⟩ := M.exists_minor_encard (Order.add_one_le_of_lt hc)
-    have : (M ／ X).RankPos := by
-      refine (eRank_ne_zero_iff (M ／ X)).mp ?_
-      simp only [hXeRK, ne_eq, add_eq_zero, ENat.coe_eq_zero, one_ne_zero, and_false,
-        not_false_eq_true]
-    exact aux (M := M ／ X) (hM.minor (contract_isMinor M X ))
-      (ht.Contract_mon hX (rankPos_nonempty)) (by simp only [hXeRK, ENat.natCast_lt_succ]) hXeRK
+  wlog hlt : M.eRk X = a + 1 generalizing M X with aux
+  · rw [←eRank_restrict] at hc
+    obtain ⟨Y, hY, hYeRK ⟩ := M.exists_minor_encard_eRk X (Order.add_one_le_of_lt hc)
+    have h1 : (M ／ Y).RankPos := by
+      refine (eRank_ne_zero_iff (M ／ Y)).mp ?_
+      have : 0 < (M ／ Y).eRank := by
+        grw [←eRk_le_eRank (M ／ Y) (X \ Y), hYeRK]
+        exact ENat.add_one_pos
+      exact Ne.symm (Std.ne_of_lt this)
+    have h3 : (X \ Y).Nonempty := by
+      by_contra hc
+      rw [nonempty_iff_ne_empty] at hc
+      simp only [ne_eq, Decidable.not_not] at hc
+      rw [hc] at hYeRK
+      simp only [eRk_empty] at hYeRK
+      have := ENat.add_one_pos (n := a)
+      grind
+    exact aux (M := M ／ Y) (X := X \ Y) (by grind ) (hM.minor (contract_isMinor M Y )) (ht.Contract_mon hY h3 )
+      (by simp only [hYeRK, ENat.natCast_lt_succ ]) hYeRK
+
   sorry
 end Thick
 
@@ -127,7 +134,7 @@ section Firm
 @[mk_iff]
 structure IsFirm (M : Matroid α) (d : ℕ∞) (X : Set (Set α)) : Prop where
   subset : ∀ x ∈ X, x ⊆ M.E
-  eRk_union : ∀ X' ⊆ X, X.encard < d * X'.encard → M.eRk (⋃₀ X) ≤ M.eRk (⋃₀ X')
+  eRk_union : ∀ X' ⊆ X, X.encard < d * X'.encard → M.eRk (⋃₀X) ≤ M.eRk (⋃₀ X')
 
 
 end Firm
